WIP

lean/FlowAnalysis/PromotionChain.lean
@@ -4,14 +4,18 @@ import Batteries.Data.List.Basic
 import Batteries.Data.List.Lemmas
 public meta import FlowAnalysis.SimpleTypes
 public import FlowAnalysis.Types
+import Mathlib.Data.Finite.Defs
+public import Mathlib.Data.Finset.Dedup
+import Mathlib.Data.Finset.Defs
+import Mathlib.Data.Set.Finite.Basic
+import Mathlib.Data.Set.Finite.Lemmas
 import Mathlib.Tactic.Order
+import Mathlib.Tactic.WLOG
 
 namespace FlowAnalysis
 
 -- Allows the use of `<+` notation for `List.Sublist`.
 open scoped List
-
-section
 
 variable {τ : Type} [DartTypeRepr τ]
 
@@ -55,18 +59,26 @@ theorem single : ∀ T : τ, isPromotionChain [T] := by
   simp [isPromotionChain]
 
 /-- The tail of a promotion chain is also a promotion chain. -/
-theorem tail_valid {ts : List τ} : isPromotionChain ts → isPromotionChain ts.tail := by
-  simp [iff_isChain]
-  intro h
-  cases ts
-  case nil => simp
-  case cons T ts' => exact List.IsChain.of_cons h
+public theorem tail_valid {T : τ} {ts : List τ} (hvalid : isPromotionChain (T::ts)) :
+    isPromotionChain ts := by
+  simp [iff_isChain] at hvalid ⊢
+  exact List.IsChain.of_cons hvalid
 
 /-- The head of a valid promotion chain is a strict supertype of every type in the tail. -/
-lemma head_bounds {T : τ} {ts : List τ} (hvalid : isPromotionChain (T::ts)) :
-    ∀ T', T' ∈ ts → T' < T := by
+public theorem head_bounds {T : τ} {ts : List τ} (hvalid : isPromotionChain (T::ts)) :
+    ∀ T' ∈ ts, T' < T := by
   simp [iff_pairwise] at hvalid
   aesop
+
+/-- The head of a valid promotion chain is not in the tail. -/
+lemma head_notIn_tail {T : τ} {ts : List τ} (hvalid : isPromotionChain (T::ts)) : T ∉ ts := by
+  have := hvalid.head_bounds T
+  grind
+
+public theorem cons {T : τ} {ts : List τ} (hbounds : ∀ T' ∈ ts, T' < T)
+    (hvalid : isPromotionChain ts) :
+    isPromotionChain (T::ts) := by
+  simp [iff_pairwise] at hvalid ⊢; grind
 
 /--
 Any sublist of a promotion chain is also a promotion chain.
@@ -91,12 +103,32 @@ local notation "PromotionChain" => PromotionChain (τ := τ)
 
 namespace «PromotionChain»
 
+@[simp]
+public theorem isValid (c : PromotionChain) : isPromotionChain c.val := c.property
+
 /-- Extensionality: promotion chains may be proven equal by proving their lists equal. -/
 public theorem ext {c₁ c₂ : PromotionChain} : c₁.val = c₂.val → c₁ = c₂ := by
   intro h; apply Subtype.ext; assumption
 
+/-- Injection: if promotion chains are equal then their values are equal. -/
+public theorem inj {c₁ c₂ : PromotionChain} : c₁ = c₂ → c₁.val = c₂.val := by
+  intro rfl; rfl
+
+/-- Equality of promotion chains may be rewritten to equality of values and vice versa. -/
+public theorem eq_iff_values_eq {c₁ c₂ : PromotionChain} : c₁ = c₂ ↔ c₁.val = c₂.val := by
+  constructor
+  · apply inj
+  · apply ext
+
 /-- The empty promotion chain. -/
 public def empty : PromotionChain := ⟨[], by simp⟩
+
+public def take (n : Nat) (c : PromotionChain) : PromotionChain := .mk (c.val.take n) $ by
+  suffices h : c.val.take n <+ c.val by apply isPromotionChain.sublist h c.property
+  exact List.take_sublist n c.val
+
+@[simp]
+public theorem take.val {n : Nat} {c : PromotionChain} : (c.take n).val = c.val.take n := by rfl
 
 public def drop (n : Nat) (c : PromotionChain) :
     PromotionChain := .mk (c.val.drop n) $ by
@@ -104,8 +136,14 @@ public def drop (n : Nat) (c : PromotionChain) :
   exact List.drop_sublist n c.val
 
 @[simp]
-public theorem drop.val {n : Nat} {c : PromotionChain} :
-    (c.drop n).val = c.val.drop n := by rfl
+public theorem drop.zero (c : PromotionChain) : drop 0 c = c := by rfl
+
+@[simp]
+public theorem drop.val {n : Nat} {c : PromotionChain} : (c.drop n).val = c.val.drop n := by rfl
+
+@[simp]
+public theorem drop.of_val {n : Nat} {c : PromotionChain} {hvalid : isPromotionChain (c.val.drop n)} :
+    ⟨c.val.drop n, hvalid⟩ = c.drop n := by rfl
 
 public instance instEmptyCollection : EmptyCollection (PromotionChain) where
   emptyCollection := empty
@@ -130,212 +168,232 @@ public theorem single_types {T : τ} : (single T).val = [T] := by rfl
 /-- A promotion chain `c` is strictly bounded by `T` iff `T::c` is a promotion chain. -/
 public def strictlyBoundedBy (c : PromotionChain) (T : τ) : Prop := isPromotionChain (T::c)
 
-@[expose]
-public def joinPromotedTypes (ts₁ ts₂ : List τ) : List τ :=
-  match ts₁, ts₂ with
-    | T₁::ts₁', T₂::ts₂' => if T₁ = T₂ then
-        T₁ :: joinPromotedTypes ts₁' ts₂'
-      else match decide (T₁ ≤ T₂), decide (T₂ ≤ T₁) with
-        | true,  true  => joinPromotedTypes ts₁' ts₂'
-        | true,  false => joinPromotedTypes (T₁::ts₁') ts₂'
-        | false, true  => joinPromotedTypes ts₁' (T₂::ts₂')
-        | false, false => []
-    | _, _ => []
+def filter (p : τ → Bool) (c : PromotionChain) : PromotionChain := .mk (c.val.filter p) $ by
+  rcases c with ⟨ts, hvalid⟩
+  rw [isPromotionChain.iff_pairwise]
+  apply List.Pairwise.filter
+  rw [←isPromotionChain.iff_pairwise]
+  simp [hvalid]
 
-@[simp]
-theorem joinPromotedTypes.idempotent (ts : List τ) :
-    joinPromotedTypes ts ts = ts := by
-  induction ts <;> simp [joinPromotedTypes]
-  case cons T ts' ih => assumption
-
-@[simp]
-public theorem joinPromotedTypes_left_empty {ts : List τ} :
-    joinPromotedTypes [] ts = [] := by
-  simp [joinPromotedTypes]
-
-@[simp]
-public theorem joinPromotedTypes_right_empty {ts : List τ} :
-    joinPromotedTypes ts [] = [] := by
-  simp [joinPromotedTypes]
-
-theorem joinPromotedTypes.commutative (ts₁ ts₂ : List τ) :
-    joinPromotedTypes ts₁ ts₂ = joinPromotedTypes ts₂ ts₁ := by
-  (cases ts₁ <;> try simp); case cons T₁ ts₁' =>
-  (cases ts₂ <;> try simp); case cons T₂ ts₂' =>
-  simp [joinPromotedTypes]
-  by_cases T₁ = T₂
-  case pos heq => subst heq; simp; apply commutative
-  case neg hne =>
-  simp [hne, Ne.symm hne]
-  by_cases T₁ ≤ T₂ <;> by_cases T₂ ≤ T₁ <;> simp_all <;> apply commutative
-
-instance joinPromotedTypes.instCommutative :
-    Std.Commutative (joinPromotedTypes (τ := τ)) where
-  comm := joinPromotedTypes.commutative
-
-@[simp]
-lemma joinPromotedTypes_sublist_left {ts₁ ts₂ : List τ} :
-    joinPromotedTypes ts₁ ts₂ <+ ts₁ := by
-  cases ts₁ <;> try simp_all
-  case cons T₁ ts₁' =>
-  cases ts₂ <;> try simp_all
-  case cons T₂ ts₂' =>
-  simp [joinPromotedTypes]
-  by_cases T₁ = T₂
-  case pos heq => simp [heq]; apply joinPromotedTypes_sublist_left
-  case neg hne =>
-  simp [hne]
-  by_cases T₂ ≤ T₁
-  case pos hge =>
-    simp [hge]
-    by_cases h : T₁ ≤ T₂ <;> simp [h] <;> calc
-      _ <+ ts₁' := by apply joinPromotedTypes_sublist_left
-      _ <+ T₁ :: ts₁' := by simp
-  case neg hnotGe =>
-    simp [hnotGe]
-    by_cases T₁ ≤ T₂
-    case pos hle => simp [hle]; apply joinPromotedTypes_sublist_left
-    case neg hnotLe => simp [hnotLe]
-
-@[simp]
-lemma joinPromotedTypes_sublist_right {ts₁ ts₂ : List τ} :
-    joinPromotedTypes ts₁ ts₂ <+ ts₂ := by
-  cases ts₁ <;> try simp_all
-  case cons T₁ ts₁' =>
-  cases ts₂ <;> try simp_all
-  case cons T₂ ts₂' =>
-  simp [joinPromotedTypes]
-  by_cases T₁ = T₂
-  case pos heq => simp [heq]; apply joinPromotedTypes_sublist_right
-  case neg hne =>
-  simp [hne]
-  by_cases T₂ ≤ T₁
-  case pos hge =>
-    simp [hge]
-    by_cases T₁ ≤ T₂
-    case pos hle => simp [hle]; calc
-      _ <+ ts₂' := by apply joinPromotedTypes_sublist_right
-      _ <+ T₂ :: ts₂' := by simp
-    case neg hnotLe => simp [hnotLe]; apply joinPromotedTypes_sublist_right
-  case neg hnotGe =>
-    simp [hnotGe]
-    by_cases T₁ ≤ T₂
-    case pos hle => simp [hle]; calc
-      _ <+ ts₂' := by apply joinPromotedTypes_sublist_right
-      _ <+ T₂ :: ts₂' := by simp
-    case neg hnotLe => simp [hnotLe]
-
-theorem isPromotionChain_join {ts₁ ts₂ : List τ} :
-    isPromotionChain ts₁ → isPromotionChain ts₂ →
-    isPromotionChain (joinPromotedTypes ts₁ ts₂) := by
-  intro hvalid₁ hvalid₂
-  apply isPromotionChain.sublist
-  case hsublist => exact joinPromotedTypes_sublist_left
-  case hvalid₂ => assumption
-
-public def join (c₁ c₂ : PromotionChain) :
-    PromotionChain :=
-  let ts := joinPromotedTypes c₁.val c₂.val
-  have hvalid : isPromotionChain ts := by
-    refine isPromotionChain_join c₁.property c₂.property
-  ⟨ts, hvalid⟩
-
-@[simp]
-public theorem join_idempotent (c : PromotionChain) :
-    c.join c = c := by
-  simp [join]
-
-@[simp]
-public theorem join.types {c₁ c₂ : PromotionChain} :
-    (c₁.join c₂).val = joinPromotedTypes c₁.val c₂.val := by
-  simp [join]
-
-/-- The join operation is idempotent (`join c c = c`). -/
-public instance instIdempotentOp_join :
-    Std.IdempotentOp (join (τ := τ)) where
-  idempotent := join_idempotent
-
-@[simp]
-public theorem join_left_empty :
-    ∀ c : PromotionChain, (∅ : PromotionChain).join c = ∅ := by
-  rintro ⟨ts, hvalid⟩
-  simp [join]
-
-@[simp]
-public theorem join_right_empty : ∀ c : PromotionChain, c.join ∅ = ∅ := by
-  rintro ⟨ts, hvalid⟩
-  simp [join]
-
-lemma bounded_skip_right {ts₁ ts₂' : List τ} {T₂ : τ}
-    (hbound : ∀ U, U ∈ ts₁ → U < T₂) :
-    joinPromotedTypes ts₁ (T₂ :: ts₂') = joinPromotedTypes ts₁ ts₂' := by
+lemma eq_if_typeSets_eq : ∀ (c₁ c₂ : PromotionChain),
+    c₁.val.toFinset = c₂.val.toFinset → c₁ = c₂ := by
+  rintro ⟨ts₁, hvalid₁⟩ ⟨ts₂, hvalid₂⟩; simp
   cases ts₁
-  case nil => simp
+  case nil => simp; intro h; rw [←List.toFinset_eq_empty_iff]; aesop
   case cons T₁ ts₁' =>
-    specialize hbound T₁ (by simp)
-    simp [joinPromotedTypes.eq_1, show T₁ ≠ T₂ by order, show T₁ ≤ T₂ by order,
-      show ¬T₂ ≤ T₁ by order]
+    cases ts₂
+    case nil => simp
+    case cons T₂ ts₂' =>
+      simp
+      by_cases T₁ = T₂
+      case pos heq =>
+        subst heq
+        intro hinsert
+        suffices h : ts₁'.toFinset = ts₂'.toFinset by
+          have := eq_if_typeSets_eq ⟨ts₁', hvalid₁.tail_valid⟩ ⟨ts₂', hvalid₂.tail_valid⟩
+          simp_all
+        simp [Finset.ext_iff] at hinsert ⊢
+        intro T; specialize hinsert T
+        by_cases T = T₁
+        case neg hne => simp [hne] at hinsert; assumption
+        case pos heq => grind [hvalid₁.head_notIn_tail, hvalid₂.head_notIn_tail]
+      case neg hne =>
+        simp [hne]; intro hcontra; simp [Finset.ext_iff] at hcontra
+        have hT₁_lt_T₂ : T₁ < T₂ := by grind [isPromotionChain.head_bounds hvalid₂]
+        have hT₂_lt_T₁ : T₂ < T₁ := by grind [isPromotionChain.head_bounds hvalid₁]
+        grind
+
+/-- Two promotion chains are equal iff they contain the same set of types. -/
+public theorem eq_iff_typeSets_eq (c₁ c₂ : PromotionChain) :
+    c₁ = c₂ ↔ c₁.val.toFinset = c₂.val.toFinset := by
+  constructor
+  · intro rfl; rfl
+  · apply eq_if_typeSets_eq
+
+public theorem eq_iff_membership (c₁ c₂ : PromotionChain) :
+    c₁ = c₂ ↔ ∀ T, T ∈ c₁.val ↔ T ∈ c₂.val := by
+  rw [eq_iff_typeSets_eq, Finset.ext_iff]; simp
 
 /--
-Equivalent formation of joinPromotedTypes, to match the current implementation. TODO(paulberry):
-make the implementation align with the definition.
+The sublist relation holds between two promotion chains iff membership in the former implies
+membership in the latter.
 -/
-public theorem joinPromotedTypes.equiv {T₁ T₂ : τ} {ts₁' ts₂' : List τ}
-    (hvalid₁ : isPromotionChain (T₁::ts₁')) :
-    joinPromotedTypes (T₁ :: ts₁') (T₂ :: ts₂') =
-      if T₁ = T₂ then T₁ :: joinPromotedTypes ts₁' ts₂'
-      else
-        match decide (T₁ ≤ T₂), decide (T₂ ≤ T₁) with
-        | true, true => joinPromotedTypes ts₁' (T₂ :: ts₂')
-        | true, false => joinPromotedTypes (T₁ :: ts₁') ts₂'
-        | false, true => joinPromotedTypes ts₁' (T₂ :: ts₂')
-        | false, false => []
-    := by
-  simp [joinPromotedTypes]
-  by_cases T₁ = T₂
-  case pos heq => simp [heq]
-  case neg hne =>
-  simp [hne]
-  by_cases T₁ ≤ T₂
-  case neg => split <;> simp_all
-  case pos hle =>
-  simp [hle]
-  by_cases T₂ ≤ T₁
-  case neg => simp_all
-  case pos hge =>
-  simp [hge]
-  suffices h : ∀ U, U ∈ ts₁' → U < T₂ by rw [bounded_skip_right h]
-  intro U U_in_ts₁'
-  calc
-    _ < T₁ := isPromotionChain.head_bounds hvalid₁ U U_in_ts₁'
-    _ ≤ T₂ := by assumption
+public theorem sublist_iff_membership (c₁ c₂ : PromotionChain) :
+    c₁.val <+ c₂.val ↔ ∀ T, T ∈ c₁.val → T ∈ c₂.val := by
+  constructor
+  · intro hsublist T hT_in_c₁
+    apply hsublist.mem; assumption
+  · intro hsubset
+    suffices c₁ = c₂.filter (· ∈ c₁.val) by rw [this]; simp [filter]
+    simp_all [eq_iff_membership, filter]
+
+public abbrev isCommonSublist (c c₁ c₂ : PromotionChain) : Prop := c.val <+ c₁.val ∧ c.val <+ c₂.val
+
+public abbrev isGreatestCommonSublist (c c₁ c₂ : PromotionChain) : Prop :=
+  c.isCommonSublist c₁ c₂ ∧ ∀ c' : PromotionChain, c'.isCommonSublist c₁ c₂ → c'.val <+ c.val
+
+-- TODO: needed?
+/-- If a type is in both c₁ and c₂, it's in a greatest common sublist. -/
+lemma isGreatestCommonSublist.mem {c c₁ c₂ : PromotionChain} :
+    c.isGreatestCommonSublist c₁ c₂ → ∀ T, T ∈ c₁.val → T ∈ c₂.val → T ∈ c.val := by
+  rintro ⟨hc_is_commonSublist, hc_is_greatest⟩ T hT_in_c₁ hT_in_c₂
+  suffices (single T).isCommonSublist c₁ c₂ by specialize hc_is_greatest (.single T) this; simp_all
+  simp_all [isCommonSublist]
+
+-- TODO: needed?
+/-- If a type is in a greatest common sublist of c₁ and c₂, then it's in c₁. -/
+lemma isGreatestCommonSublist.mem_left {c c₁ c₂ : PromotionChain} {T : τ} :
+    c.isGreatestCommonSublist c₁ c₂ → T ∈ c.val → T ∈ c₁.val := by grind
+
+-- TODO: needed?
+/-- If a type is in a greatest common sublist of c₁ and c₂, then it's in c₂. -/
+lemma isGreatestCommonSublist.mem_right {c c₁ c₂ : PromotionChain} {T : τ} :
+    c.isGreatestCommonSublist c₁ c₂ → T ∈ c.val → T ∈ c₂.val := by grind
+
+/-- The unique greatest common sublist of two promotion chains is called their `join`. -/
+public def join (c₁ c₂ : PromotionChain) := c₁.filter (· ∈ c₂.val)
+
+theorem join.spec (c₁ c₂ : PromotionChain) : (c₁.join c₂).isGreatestCommonSublist c₁ c₂ := by
+  simp [join]
+  constructor
+  · constructor
+    · simp [filter]
+    · rw [sublist_iff_membership]; simp [filter]
+  · rintro c' ⟨hc'_sublist_c₁, hc'_sublist_c₂⟩
+    rw [sublist_iff_membership] at hc'_sublist_c₁ hc'_sublist_c₂ ⊢
+    intro T hT_in_c'
+    simp [filter, hc'_sublist_c₁ T hT_in_c', hc'_sublist_c₂ T hT_in_c']
+
+/--
+The computable definition of `join` above proves that a greatest common sublist always exists.
+-/
+lemma greatestCommonSublist_exists (c₁ c₂ : PromotionChain) :
+    ∃ c : PromotionChain, c.isGreatestCommonSublist c₁ c₂ := by
+  exists c₁.filter (· ∈ c₂.val)
+  apply join.spec
+
+/-- The join is the unique greatest common sublist. -/
+public theorem greatestCommonSublist_unique (c₁ c₂ : PromotionChain) :
+    ∀ c : PromotionChain, c.isGreatestCommonSublist c₁ c₂ → c = c₁.join c₂ := by
+  intro c hc
+  let c' := c₁.join c₂
+  have hc' := join.spec c₁ c₂
+  rw [eq_iff_membership]; grind
+
+@[simp]
+public theorem join.membership (c₁ c₂ : PromotionChain) (T : τ) :
+    T ∈ (c₁.join c₂).val ↔ T ∈ c₁.val ∧ T ∈ c₂.val := by
+  obtain ⟨⟨hjoin_sublist_c₁, hjoin_sublist_c₂⟩, hgreatest⟩ := join.spec c₁ c₂
+  rw [PromotionChain.sublist_iff_membership] at hjoin_sublist_c₁ hjoin_sublist_c₂
+  constructor
+  · grind
+  · simp; intro hT_in_c₁ hT_in_c₂
+    specialize hgreatest (.single T) (by simp_all [isCommonSublist])
+    rw [PromotionChain.sublist_iff_membership] at hgreatest; simp at hgreatest; assumption
+
+public theorem join.eq_iff (c c₁ c₂ : PromotionChain) :
+    c₁.join c₂ = c ↔ ∀ T, T ∈ c₁.val ∧ T ∈ c₂.val ↔ T ∈ c.val := by
+  constructor
+  · intro rfl T; simp
+  · rw [eq_iff_membership]; simp
+
+@[simp]
+public theorem join.sublist_left (c₁ c₂ : PromotionChain) :
+    c₁.val <+ c₂.val → c₁.join c₂ = c₁ := by
+  intro h; rw [eq_iff]; intro T; grind
+
+@[simp]
+public theorem join.sublist_right (c₁ c₂ : PromotionChain) :
+    c₂.val <+ c₁.val → c₁.join c₂ = c₂ := by
+  intro h; rw [eq_iff]; intro T; grind
+
+/-- The join operation is idempotent (`join c c = c`). -/
+@[simp]
+public theorem join.idempotent (c : PromotionChain) : c.join c = c := by
+  rw [eq_iff]; grind
+
+public instance join.instIdempotentOp :
+    Std.IdempotentOp (join (τ := τ)) where
+  idempotent := idempotent
+
+/-- The join operation is commutative (`c₁.join c₂ = c₂.join c₁`). -/
+public theorem join.commutative (c₁ c₂ : PromotionChain) : c₁.join c₂ = c₂.join c₁ := by
+  rw [eq_iff_membership]; simp; aesop
+
+public instance join.instCommutative : Std.Commutative (join (τ := τ)) where
+  comm := commutative
+
+/-- The join operation is associative (`(c₁.join c₂).join c₃ = c₁.join (c₂.join c₃)`) -/
+public theorem join.associative (c₁ c₂ c₃ : PromotionChain) :
+    (c₁.join c₂).join c₃ = c₁.join (c₂.join c₃) := by
+  rw [eq_iff_membership]; simp; aesop
+
+public instance join.instAssociative : Std.Associative (join (τ := τ)) where
+  assoc := associative
+
+@[simp]
+public theorem join.left_empty :
+    ∀ c : PromotionChain, (∅ : PromotionChain).join c = ∅ := by
+  intro c; rw [eq_iff]; simp
+
+@[simp]
+public theorem join.right_empty : ∀ c : PromotionChain, c.join ∅ = ∅ := by
+  intro c; rw [eq_iff]; simp
+
+-- TODO: needed?
+lemma filter_refineGuard_notIn {α} {P : α → Bool} {l : List α} {y : α} [DecidableEq α] : y ∉ l →
+    List.filter (fun x => decide (x = y) || P x) l =
+    List.filter (fun x => P x) l := by
+  intro h; apply List.filter_congr; simp; intro x hx_in_l rfl; contradiction
+
+@[simp]
+lemma join.heads_eq_valid {T : τ} {ts₁' ts₂' : List τ}
+    {hvalid₁ : isPromotionChain (T::ts₁')} {hvalid₂ : isPromotionChain (T::ts₂')} :
+    isPromotionChain (T :: join ⟨ts₁', hvalid₁.tail_valid⟩ ⟨ts₂', hvalid₂.tail_valid⟩) := by
+  apply isPromotionChain.cons <;> simp
+  intro T' hT'_in_ts₁' hT'_in_ts₂'
+  apply hvalid₁.head_bounds; assumption
+
+@[simp]
+public theorem join.heads_eq {T : τ} {ts₁' ts₂' : List τ}
+    {hvalid₁ : isPromotionChain (T::ts₁')} {hvalid₂ : isPromotionChain (T::ts₂')} :
+    join ⟨T::ts₁', hvalid₁⟩ ⟨T::ts₂', hvalid₂⟩ =
+    ⟨T :: join ⟨ts₁', hvalid₁.tail_valid⟩ ⟨ts₂', hvalid₂.tail_valid⟩, by simp_all⟩ := by
+  rw [eq_iff_membership]; intro T'
+  constructor <;> simp <;> grind
+
+@[simp]
+public theorem join.heads_ne_le {T₁ T₂ : τ} {ts₁' ts₂' : List τ}
+    {hvalid₁ : isPromotionChain (T₁::ts₁')} {hvalid₂ : isPromotionChain (T₂::ts₂')}
+    (hne : ¬T₁ = T₂) (hle : T₁ ≤ T₂) :
+    join ⟨T₁::ts₁', hvalid₁⟩ ⟨T₂::ts₂', hvalid₂⟩ =
+    join ⟨T₁::ts₁', hvalid₁⟩ ⟨ts₂', hvalid₂.tail_valid⟩ := by
+  rw [eq_iff_membership]; intro T; simp
+  intro h rfl; simp [show T = T₁ ↔ False by grind] at h
+  have := hvalid₁.head_bounds T h
+  grind
+
+@[simp]
+public theorem join.heads_ne_notLe {T₁ T₂ : τ} {ts₁' ts₂' : List τ}
+    {hvalid₁ : isPromotionChain (T₁::ts₁')} {hvalid₂ : isPromotionChain (T₂::ts₂')}
+    (hne : ¬T₁ = T₂) (hnotLe : ¬T₁ ≤ T₂) :
+    join ⟨T₁::ts₁', hvalid₁⟩ ⟨T₂::ts₂', hvalid₂⟩ =
+    join ⟨ts₁', hvalid₁.tail_valid⟩ ⟨T₂::ts₂', hvalid₂⟩ := by
+  rw [eq_iff_membership]; intro T; simp
+  intro h rfl; simp [show T = T₂ ↔ False by grind] at h
+  have := hvalid₂.head_bounds T h
+  grind
+
+@[grind =>]
+public theorem val_notEmpty_if_notEmpty {c : PromotionChain} : ¬c = ∅ → ¬c.val = [] := by
+  contrapose; rcases c; simp; intro rfl; simp
+
+@[simp]
+public theorem join.left_empty' {c₁ c₂ : PromotionChain} : c₁.val = [] → c₁.join c₂ = ∅ := by
+  intro h; simp [show c₁ = ∅ by grind]
+
+@[simp]
+public theorem join.right_empty' {c₁ c₂ : PromotionChain} : c₂.val = [] → c₁.join c₂ = ∅ := by
+  intro h; simp [show c₂ = ∅ by grind]
 
 end «PromotionChain»
-end
-
-section
-
-/-- The join operation is *not* associative. -/
-public theorem PromotionChain.join_not_associative :
-    ¬∀ (τ : Type) [DartTypeRepr τ] (c₁ c₂ c₃ : PromotionChain (τ := τ)),
-      (c₁.join c₂).join c₃ = c₁.join (c₂.join c₃) := by
-  let Γ : DartTypeRepr SimpleType := inferInstance
-  let c₁ : PromotionChain := ⟨[Γ.Map Γ.ObjectQ Γ.int, Γ.Map Γ.int Γ.int],
-    by simp [isPromotionChain.iff_isChain, SimpleType.isSubtype]⟩
-  let c₂ : PromotionChain := ⟨[Γ.Map Γ.dynamic Γ.int, Γ.Map Γ.int Γ.int],
-    by simp [isPromotionChain.iff_isChain, SimpleType.isSubtype]⟩
-  let c₃ : PromotionChain := ⟨[Γ.Map Γ.int Γ.Object, Γ.Map Γ.int Γ.int],
-    by simp [isPromotionChain.iff_isChain, SimpleType.isSubtype]⟩
-  let c₁₂ : PromotionChain := ⟨[Γ.Map Γ.int Γ.int], by simp⟩
-  intro h
-  specialize h SimpleType c₁ c₂ c₃
-  rw [show c₁.join c₂ = c₁₂ by simp [c₁, c₂, c₁₂, PromotionChain.join,
-    PromotionChain.joinPromotedTypes, SimpleType.isSubtype]] at h
-  rw [show c₁₂.join c₃ = c₁₂ by simp [c₁₂, c₃, PromotionChain.join,
-    PromotionChain.joinPromotedTypes, SimpleType.isSubtype]] at h
-  rw [show c₂.join c₃ = ∅ by simp [c₂, c₃, PromotionChain.join,
-    PromotionChain.joinPromotedTypes, SimpleType.isSubtype]] at h
-  rw [show c₁.join ∅ = ∅ by simp] at h
-  injection h; contradiction
-
-end
