lean/FlowAnalysis.lean
@@ -2,3 +2,9 @@ module
 public import FlowAnalysis.PromotionChain
 public import FlowAnalysis.SimpleTypes
 public import FlowAnalysis.Types
+public import FlowAnalysis.Syntax
+public import FlowAnalysis.Lowered
+public import FlowAnalysis.State
+public import FlowAnalysis.Elaboration
+public import FlowAnalysis.Algorithm
+public import FlowAnalysis.AlgorithmTheorems
