lean/FlowAnalysis/Algorithm.lean
@@ -1,0 +1,232 @@
+/-
+This module contains an algorithmic implementation of the flow analysis rules defined in
+`FlowAnalysis.Elaboration`.
+-/
+
+module
+public import Std.Data.HashMap
+import FlowAnalysis.Elaboration
+public import FlowAnalysis.Lowered
+public import FlowAnalysis.State
+public import FlowAnalysis.Syntax
+public import FlowAnalysis.Types
+
+open FlowAnalysis
+
+namespace FlowAnalysis
+
+open DartTypeRepr
+
+variable {τ : Type} [Γ : DartTypeRepr τ]
+
+local notation "Expr" => Expr (τ := τ)
+local notation "LoweredExpr" => LoweredExpr (τ := τ)
+local notation "Reference" => Reference (τ := τ)
+local notation "Stmt" => Stmt (τ := τ)
+local notation "Variable" => Variable (τ := τ)
+
+public structure ValueModelA where
+  promotedTypes : List τ
+
+local notation "ValueModelA" => ValueModelA (τ := τ)
+
+/--
+If `a?` is `some a`, returns the value `a`. Otherwise throws an exception.
+-/
+@[expose]
+public def _root_.Option.assert {m α} [Monad m] [MonadExcept String m] (a? : Option α) : m α :=
+  match a? with
+    | none => throw "No value"
+    | some a => pure a
+
+@[expose]
+public def joinPromotedTypesA' {m} [Monad m] [MonadExcept String m] (ts₁ ts₂ : List τ) :
+    m (List τ) := do
+  let mut i₁ := 0
+  let mut i₂ := 0
+  let mut T₁ ← ts₁[0]?.assert
+  let mut T₂ ← ts₂[0]?.assert
+  let mut result : Option (List τ) := none
+  repeat do
+    let mut advance_i₁ : Option Bool := none
+    let mut advance_i₂ : Option Bool := none
+    if T₁ = T₂ then
+      result := result.map (· ++ [T₁])
+      advance_i₁ := true
+      advance_i₂ := true
+    else if T₁ ≤ T₂ then
+      advance_i₁ := false
+      advance_i₂ := true
+    else
+      result := result.getD (ts₁.take i₁)
+      advance_i₁ := true
+      advance_i₂ := false
+    if ←advance_i₁.assert then
+      i₁ := i₁ + 1
+      if i₁ = ts₁.length then
+        if result ≠ none then return ←result.assert
+        return ts₁
+      T₁ ← ts₁[i₁]?.assert
+    if ←advance_i₂.assert then
+      i₂ := i₂ + 1
+      if i₂ = ts₂.length then
+        if result ≠ none then return ←result.assert
+        if i₁ = ts₁.length then return ts₁
+        return ts₁.take i₁
+      T₂ ← ts₂[i₂]?.assert
+
+@[expose]
+public def joinPromotedTypesA {m} [Monad m] [MonadExcept String m] (ts₁ ts₂ : List τ) :
+    m (List τ) := do
+  let mut ts₁ := ts₁
+  let mut ts₂ := ts₂
+  if ts₁ = [] then return ts₁
+  if ts₂ = [] then return ts₂
+  if ts₁.length > ts₂.length then
+    let tmp := ts₁
+    ts₁ := ts₂
+    ts₂ := tmp
+  joinPromotedTypesA' ts₁ ts₂
+
+/-- Not exposed so that proofs can't rely on it -/
+public def unspecifiedPromotionChain : List τ := []
+
+@[expose]
+public def ValueModelA.join (vmA₁ vmA₂ : ValueModelA) : ValueModelA :=
+  match (joinPromotedTypesA vmA₁.promotedTypes vmA₂.promotedTypes : ExceptT String Id _).run with
+    | .ok ts => ⟨ts⟩
+    | .error _ => ⟨unspecifiedPromotionChain⟩
+
+@[expose]
+public def ValueModelA.promotedType? (vmA : ValueModelA) : Option τ :=
+  vmA.promotedTypes.getLast?
+
+@[expose]
+public def ValueModelA.currentType (vmA : ValueModelA) (baseType : τ) :
+    τ :=
+  match vmA.promotedType? with
+  | none => baseType
+  | some T => if T ≤ baseType then T else baseType
+
+-- TODO: use a more PromotionInfo-like structure
+public structure FlowModelA where
+  env : Std.HashMap Variable ValueModelA
+deriving Inhabited
+
+local notation "FlowModelA" => FlowModelA (τ := τ)
+
+@[expose]
+public def FlowModelA.empty : FlowModelA := ⟨∅⟩
+
+@[expose]
+public def mergeMaps {α β : Type} [BEq α] [Hashable α]
+    (f : β → β → β) (m₁ m₂ : Std.HashMap α β) : Std.HashMap α β :=
+  m₁.filterMap fun k v₁ =>
+    match m₂[k]? with
+     | none => none
+     | some v₂ => f v₁ v₂
+
+@[expose]
+public def FlowModelA.join (fmA₁ fmA₂ : FlowModelA) :
+    FlowModelA :=
+  -- TODO: reachability
+  -- TODO: identical check
+  if fmA₁.env.isEmpty then fmA₁ else
+  if fmA₂.env.isEmpty then fmA₂ else
+  ⟨mergeMaps ValueModelA.join fmA₁.env fmA₂.env⟩
+
+public structure ExprModelA where
+  type : τ
+  ref? : Option Reference
+  boolInfo : Option (FlowModelA × FlowModelA)
+
+local notation "ExprModelA" => ExprModelA (τ := τ)
+
+public structure Config where
+
+/--
+Elaboration algorithms are defined using a state monad that records the current flow analysis
+state. This state is updated as we recursively traverse the code being analyzed.
+-/
+public abbrev AlgM :=
+  ReaderT Config (StateT FlowModelA (ExceptT String Id))
+
+local notation "AlgM" => AlgM (τ := τ)
+
+@[expose]
+public def tryPromoteA (ref : Option Reference) (T : τ) :
+    AlgM Unit := do
+  match ref with
+  | some (Reference.var v) =>
+    match (<- get).env[v]? with
+    | some vmA =>
+      if T < vmA.currentType v.type then
+        modify (fun s => { s with env := s.env.insert v ⟨[T]⟩})
+    | none => pure ()
+  | none => pure ()
+
+mutual
+
+@[expose]
+public def elabExprA (e : Expr) :
+    AlgM
+      (LoweredExpr × ExprModelA) := do
+  match e with
+  | .var v =>
+    match (<- get).env[v]? with
+    | some vm =>
+        let T := vm.currentType v.type
+        pure (LoweredExpr.var v T, ⟨T, some (Reference.var v), none⟩)
+    | none => throw s!"Undefined variable {v.name}"
+  | .nullCheck eInner =>
+    let (m, emA) <- elabExprA eInner
+    let T' := NonNull emA.type
+    tryPromoteA emA.ref? T'
+    pure (m.nullCheck, ⟨T', none, none⟩)
+  | .as eInner T =>
+    let (m, emA) <- elabExprA eInner
+    tryPromoteA emA.ref? T
+    pure (m.as T, ⟨T, none, none⟩)
+  | .null =>
+    pure (.null, ⟨Γ.Null, none, none⟩)
+
+public def elabStmtA (s : Stmt) :
+    AlgM LoweredExpr := do
+  match s with
+  | .declare n T =>
+    modify (fun s => { s with env := s.env.insert ⟨n, T⟩ ⟨[]⟩ })
+    pure (LoweredExpr.declare ⟨n, T⟩ T)
+  | .exprStmt e =>
+    let (m, _) <- elabExprA e
+    pure m
+  | .ifStmt e₁ s₂ s₃ =>
+    let (m₁, em₁) <- elabExprA e₁
+    -- TODO: handle dynamic
+    if em₁.type != Γ.bool then throw s!"Type of {e₁} is {em₁.type}, expected bool" else
+    -- TODO: make a helper function for some of this logic?
+    let fm₁ <- get
+    let (fm₁_true, fm₁_false) := em₁.boolInfo.getD (fm₁, fm₁)
+    set fm₁_true
+    let m₂ <- elabStmtA s₂
+    let fm₂ <- get
+    set fm₁_false
+    let m₃ <- elabStmtA s₃
+    let fm₃ <- get
+    set (fm₂.join fm₃)
+    pure (.cond m₁ m₂ m₃ Γ.Null)
+  | .block stmts =>
+    let loweredStmts <- elabStmtsA stmts
+    pure (LoweredExpr.block loweredStmts)
+
+public def elabStmtsA (ss : List Stmt) :
+    AlgM (List LoweredExpr) := do
+  match ss with
+  | [] => pure []
+  | s :: ss' =>
+    let loweredS <- elabStmtA s
+    let loweredSS <- elabStmtsA ss'
+    pure (loweredS :: loweredSS)
+
+end
+
+end FlowAnalysis
