lean/FlowAnalysis/AlgorithmTheorems.lean
@@ -1,0 +1,1073 @@
+/-
+Proofs of soundness and completeness of the algorithmic implementation in `FlowAnalysis.algorithm`.
+-/
+
+module
+import Aesop
+public import Lean
+import Mathlib.Logic.Basic
+import Mathlib.Tactic.Cases
+import Mathlib.Tactic.GRewrite
+import Mathlib.Tactic.SplitIfs
+import Std.Data.HashMap
+import Std.Tactic.Do
+import FlowAnalysis.Algorithm
+import FlowAnalysis.Elaboration
+import Mathlib.Tactic.Order
+
+section
+open Lean Elab Tactic Meta
+
+/--
+`by_cases_iff h` splits a hypothesis `h : P ↔ Q` into two subgoals:
+- `pos`: assuming both `P` and `Q` are true.
+- `neg`: assuming both `¬P` and `¬Q` are true.
+-/
+elab "by_cases_iff" t:term : tactic => withMainContext do
+  -- 1. Split the equivalence: creates a temporary `Or` hypothesis and case-splits it
+  evalTactic (← `(tactic| have h_or := iff_iff_and_or_not_and_not.mp $t))
+  evalTactic (← `(tactic| cases h_or <;> rename_i h_or <;> cases h_or))
+
+  -- 2. Grab the two resulting subgoals and assign the `pos` and `neg` tags
+  let goals ← getGoals
+  match goals with
+  | g1 :: g2 :: rest =>
+    g1.setTag `pos
+    g2.setTag `neg
+    setGoals (g1 :: g2 :: rest)
+  | _ =>
+    -- Fail silently or log nothing if the goal was solved during splitting
+    pure ()
+end
+
+namespace FlowAnalysis
+
+open DartTypeRepr
+
+-- Allows the use of `<+` notation for `List.Sublist`.
+-- TODO: needed?
+open scoped List
+
+variable {τ : Type} [Γ : DartTypeRepr τ]
+variable {cfg : Config}
+
+local notation "AlgM" => AlgM (τ := τ)
+local notation "Expr" => Expr (τ := τ)
+local notation "ExprModel" => ExprModel (τ := τ)
+local notation "ExprModelA" => ExprModelA (τ := τ)
+local notation "FlowModel" => FlowModel (τ := τ)
+local notation "FlowModelA" => FlowModelA (τ := τ)
+local notation "PromotionChain" => PromotionChain (τ := τ)
+local notation "Stmt" => Stmt (τ := τ)
+local notation "ValueModel" => ValueModel (τ := τ)
+local notation "ValueModelA" => ValueModelA (τ := τ)
+
+theorem AlgM_get_eq {fm} :
+  (get : AlgM _) cfg fm = Except.ok (fm, fm) := rfl
+
+theorem AlgM_pure_eq {α fm} {a : α} :
+  (pure a : AlgM _) cfg fm = Except.ok (a, fm) := rfl
+
+theorem AlgM_bind_eq {α β : Type} {x : AlgM α} {fm : FlowModelA}
+    {f : α → AlgM β} :
+  (x >>= f) cfg fm = match x cfg fm with
+                 | Except.ok (a, hm') => f a cfg hm'
+                 | Except.error e => Except.error e := by
+  simp [bind, ReaderT.bind, StateT.bind]
+  cases x cfg fm <;> rfl
+
+theorem AlgM_map_eq {α β : Type} {fm : FlowModelA} {f : α → β} {x : AlgM α} :
+  (f <$> x) cfg fm = match x cfg fm with
+                 | Except.ok (a, hm') => Except.ok (f a, hm')
+                 | Except.error e => Except.error e := by
+  dsimp [Functor.map, StateT.instMonad, StateT.map, StateT.bind, StateT.pure, ExceptT.bind, ExceptT.pure, bind, pure]
+  cases x cfg fm <;> trivial
+
+theorem AlgM_modify_eq {f fm} :
+    (modify : _ → AlgM _) f cfg fm = Except.ok ((), f fm) := rfl
+
+theorem AlgM_set_eq {fm fm'} :
+    (set : _ → AlgM _) fm' cfg fm = Except.ok ((), fm') := rfl
+
+theorem AlgM_throw_eq_ok_contra {α e fmA₀ x fmA} :
+    (throw e : AlgM α) cfg fmA₀ = Except.ok (x, fmA) ↔ False := by
+  constructor
+  case mp => intro h; contradiction
+  case mpr => intro h; exfalso; assumption
+
+structure ValueModelA.refines (vmA : ValueModelA) (vm : ValueModel) :
+    Prop where
+  types : vmA.promotedTypes = vm.promotedTypes.val
+
+theorem ValueModelA.refines.unique {vmA : ValueModelA}
+    {vm₁ vm₂ : ValueModel} :
+    vmA.refines vm₁ → vmA.refines vm₂ → vm₁ = vm₂ := by
+  intro h₁ h₂
+  ext
+  rw [←h₁.types, ←h₂.types]
+
+@[simp]
+theorem ValueModelA.refines.empty :
+    (⟨[]⟩ : ValueModelA).refines ⟨∅⟩ := by
+  constructor
+  · simp
+
+-- TODO: remove when no longer needed
+@[simp]
+theorem ValueModelA.refines.single {T : τ} :
+    (⟨[T]⟩ : ValueModelA).refines ⟨.single T⟩ := by
+  constructor
+  · simp
+
+theorem ValueModelA.refines.currentTypes {vmA : ValueModelA} {vm : ValueModel} {baseType : τ} :
+    vmA.refines vm → vmA.currentType baseType = vm.currentType baseType := by
+  intro hrefines
+  simp [ValueModelA.currentType, ValueModelA.promotedType?, ValueModel.currentType]
+  rw [hrefines.types]
+  rfl
+
+section
+open FlowAnalysis.ValueModelA
+open FlowAnalysis.PromotionChain
+open Std.Do
+
+-- TODO: remove?
+lemma split_chain_at_index {i : Nat} {c : PromotionChain} (h : i < c.val.length) :
+    ∃ (c' : PromotionChain) (x : τ) (c'' : PromotionChain) (hbounds : ∀ T' ∈ c''.val, T' < x),
+      c.val[i] = x ∧
+      c.val.take i = c'.val ∧
+      c.val.take (i + 1) = c'.val ++ [x] ∧
+      c.drop i = ⟨x::c''.val, isPromotionChain.cons hbounds c''.property⟩ ∧
+      c.drop (i + 1) = c'' := by
+  exists c.take i, c.val[i], c.drop (i + 1)
+  exists by
+    apply isPromotionChain.head_bounds
+    suffices c.val[i] :: (c.drop (i + 1)).val = (c.drop i).val by
+      rw [this]; apply (c.drop i).property
+    simp
+  simp
+
+def stateIs {σs} (s : SVal.StateTuple σs) : SPred σs := SVal.curry (fun s' => ⟨s' = s⟩)
+
+-- TODO: needed?
+def currentIs (fmA : FlowModelA) :
+    SPred [Config, FlowModelA] :=
+  (SVal.getThe FlowModelA).evalsTo fmA
+
+@[simp]
+theorem curry_evalsTo_pure :
+    (((SVal.curry fun _ => ULift.up v)).evalsTo (ULift.up v') : SPred σs) = ⌜v = v'⌝ := by
+  apply SPred.bientails.to_eq
+  induction σs
+  case nil => grind
+  case cons σ σs' ih => intro s; simp; assumption
+
+-- TODO: rename and move to PromotionChain.lean if needed
+lemma foo {c : PromotionChain} {ts : List τ} : c.val = ts → ∃ hvalid, c = ⟨ts, hvalid⟩ := by
+  intro rfl; exists c.property
+
+-- TODO: move to PromotionChain.lean if needed
+lemma PromotionChain.membership_if_value_eq {c : PromotionChain} {ts : List τ} :
+    c.val = ts → ∀ T, T ∈ c.val ↔ T ∈ ts := by
+  intro rfl T; simp
+
+-- TODO: maybe just go back to doing a normal split since I'm not trying to avoid simp anymore.
+lemma WP_ite [Monad m] [WP m ps] {t e : m α} [Decidable c] (hifTrue : c → P ⊢ₛ wp⟦t⟧ Q)
+    (hifFalse : ¬c → P ⊢ₛ wp⟦e⟧ Q) : P ⊢ₛ wp⟦if c then t else e⟧ Q := by
+  mintro hP
+  split
+  case isTrue h => apply hifTrue h
+  case isFalse h => apply hifFalse h
+
+-- TODO: not sure I like this.
+--theorem assert_spec {m ps α} {v : Option α} {s₀ a} [Monad m] [MonadExcept String m] [WPMonad m ps] :
+--    ⦃stateIs s₀ ∧ ⌜v = some a⌝⦄ (Option.assert v : m _) ⦃⇓ r => stateIs s₀ ∧ ⌜r = a⌝⦄ := by
+--  mintro h; mcases h with ⟨hstate, hv⟩; subst hv
+--  unfold Option.assert; simp
+--  mconstructor; massumption; mpure_intro; trivial
+
+@[simp]
+theorem assert_rw [Monad m] [MonadExcept String m] :
+    (Option.assert (some x) : m _) = pure x := by rfl
+
+lemma bar {i T} {c : PromotionChain} (hrange : i < c.val.length) (hT : T = c.val[i]) : ∃ hvalid,
+    c.drop i = ⟨T :: c.drop (i+1), hvalid⟩ := by
+  rcases c with ⟨ts, hvalid⟩; simp_all
+
+lemma baz {m α} {i : Nat} {ts : List α} [Monad m] [MonadExcept String m] (hrange: i < ts.length) :
+  ts[i]?.assert = (pure ts[i] : m _) := by simp_all [Option.assert]
+
+theorem joinPromotedTypesA'_correct [Monad m] [MonadExcept String m] [Lean.Order.MonadTail m]
+    [WPMonad m ps] (c₁ c₂ : PromotionChain) :
+    0 < c₁.val.length → c₁.val.length ≤ c₂.val.length → ⦃stateIs s₀⦄ (joinPromotedTypesA' c₁.val c₂.val : m _)
+    ⦃⇓ r => stateIs s₀ ∧ ⌜r = (c₁.join c₂).val⌝⦄ := by
+  intro hc₁_nonEmpty hc₁_smaller
+  mintro hstate
+  unfold joinPromotedTypesA'
+  rw [baz hc₁_nonEmpty, baz (by order)]
+  simp
+  mspec Spec.forIn_loop
+  case measure => exact fun vars => SVal.curry fun _ => ⟨match vars with
+    | ⟨_, i₁, i₂, _⟩ => c₁.val.length + c₂.val.length - i₁ - i₂
+  ⟩
+  case inv => exact (⇓ cursor => (match cursor with
+    | .inl (retval, i₁, i₂, T₁, T₂, result) =>
+      spred(stateIs s₀ ∧ ⌜retval = none ∧ (∃ hrange₁ : i₁ < c₁.val.length, T₁ = c₁.val[i₁]) ∧
+        (∃ hrange₂ : i₂ < c₂.val.length, T₂ = c₂.val[i₂]) ∧
+        (c₁.join c₂).val =
+          retval.getD (result.getD (c₁.val.take i₁) ++ (c₁.drop i₁).join (c₂.drop i₂))⌝)
+    | .inr (retval, i₁, i₂, T₁, T₂, result) =>
+      spred(stateIs s₀ ∧ ⌜retval = some (c₁.join c₂).val⌝)
+    ))
+  case step =>
+    simp; intro retval i₁ i₂ T₁ T₂ result mb
+    mintro h; mcases h with ⟨hmb, hstate, h⟩; rcases h with
+      ⟨rfl, ⟨hrange₁, hT₁⟩, ⟨hrange₂, hT₂⟩, hjoin⟩; simp at hjoin
+    split
+    case isTrue heq =>
+      subst heq
+      -- T₁ belongs in the output, so we can rewrite hjoin.
+      have hT₁_belongs : (c₁.drop i₁).join (c₂.drop i₂) =
+          T₁ :: (c₁.drop (i₁+1)).join (c₂.drop (i₂+1)) := by
+        obtain ⟨hvalid_drop₁, hdrop₁⟩ := bar hrange₁ hT₁; rw [hdrop₁]
+        obtain ⟨hvalid_drop₂, hdrop₂⟩ := bar hrange₂ hT₂; rw [hdrop₂]
+        simp
+      rw [hT₁_belongs] at hjoin; clear hT₁_belongs
+      split
+      case isTrue hdone₁ =>
+        rw [hdone₁] at hjoin; simp at hjoin; split
+        case isTrue hresult =>
+          subst hresult; simp [hT₁] at hjoin ⊢; rw [hdone₁] at hjoin; simp at hjoin
+          mconstructor; massumption; mpure_intro; aesop
+        case isFalse hresult =>
+          rcases result; contradiction; rename_i result; clear hresult; simp at hjoin
+          simp; mconstructor; massumption; mpure_intro; aesop
+      case isFalse hrange₁ =>
+        replace hrange₁ : i₁ + 1 < c₁.val.length := by grind
+        rw [baz hrange₁]; simp
+        split
+        case isTrue hdone₂ =>
+          rw [hdone₂] at hjoin; simp at hjoin; split
+          case isTrue hresult =>
+            subst hresult; simp [hT₂] at hjoin ⊢
+            mconstructor; massumption; mpure_intro
+            rw [show c₁.val.take (i₁+1) = c₁.val.take i₁ ++ [T₁] by simp_all, hT₂]; aesop
+          case isFalse hresult =>
+            rcases result; contradiction; rename_i result _; clear hresult; simp at hjoin ⊢
+            mconstructor; massumption; mpure_intro; aesop
+        case isFalse hrange₂ =>
+          replace hrange₂ : i₂ + 1 < c₂.val.length := by grind
+          simp; rw [baz hrange₂]; simp
+          mexists c₁.val.length + c₂.val.length - (i₁ + 1) - (i₂ + 1); simp
+          mconstructor; · mpure_intro; trivial
+          mconstructor; · mpure_intro; grind
+          mconstructor; massumption; mpure_intro
+          constructor; · assumption
+          constructor; assumption
+          cases result
+          case none =>
+            simp at hjoin ⊢
+            rw [show c₁.val.take (i₁+1) = c₁.val.take i₁ ++ [T₁] by simp_all]; simp; assumption
+          case some result => simp at hjoin ⊢; assumption
+    case isFalse hne =>
+      split
+      case isTrue hle =>
+        -- T₂ does not belong in the output, so we can rewrite hjoin.
+        have hT₂_notBelongs : (c₁.drop i₁).join (c₂.drop i₂) =
+            (c₁.drop i₁).join (c₂.drop (i₂+1)) := by
+          obtain ⟨hvalid_drop₁, hdrop₁⟩ := bar hrange₁ hT₁; rw [hdrop₁]
+          obtain ⟨hvalid_drop₂, hdrop₂⟩ := bar hrange₂ hT₂; rw [hdrop₂]
+          simp [hne, hle]
+        rw [hT₂_notBelongs] at hjoin; clear hT₂_notBelongs
+        split
+        case isTrue hdone₂ =>
+          rw [hdone₂] at hjoin; simp at hjoin; split
+          case isTrue hresult =>
+            subst hresult; simp [hT₁] at hjoin ⊢
+            split
+            case isTrue hrange₁ => simp; mconstructor; massumption; mpure_intro; simp_all
+            case isFalse hrange₁ => simp; mconstructor; massumption; mpure_intro; aesop
+          case isFalse hresult =>
+            rcases result; contradiction; rename_i result; clear hresult; simp at hjoin
+            simp; mconstructor; massumption; mpure_intro; aesop
+        case isFalse hrange₂ =>
+          replace hrange₂ : i₂ + 1 < c₂.val.length := by grind
+          simp; rw [baz hrange₂]; simp
+          mexists c₁.val.length + c₂.val.length - i₁ - (i₂ + 1)
+          mconstructor; · mpure_intro; trivial
+          mconstructor; · mpure_intro; grind
+          mconstructor; massumption; mpure_intro
+          constructor; · exists hrange₁
+          constructor; · assumption
+          cases result
+          case none => simp at hjoin ⊢; assumption
+          case some result => simp at hjoin ⊢; assumption
+      case isFalse hnotLe =>
+        -- T₁ does not belong in the output, so we can rewrite hjoin.
+        have hT₁_notBelongs : (c₁.drop i₁).join (c₂.drop i₂) =
+            (c₁.drop (i₁+1)).join (c₂.drop i₂) := by
+          obtain ⟨hvalid_drop₁, hdrop₁⟩ := bar hrange₁ hT₁; rw [hdrop₁]
+          obtain ⟨hvalid_drop₂, hdrop₂⟩ := bar hrange₂ hT₂; rw [hdrop₂]
+          simp [hne, hnotLe]
+        rw [hT₁_notBelongs] at hjoin; clear hT₁_notBelongs
+        split
+        case isTrue hdone₁ =>
+          rw [hdone₁] at hjoin; simp at hjoin ⊢
+          mconstructor; massumption; mpure_intro; aesop
+        case isFalse hrange₁ =>
+          replace hrange₁ : i₁ + 1 < c₁.val.length := by grind
+          simp; rw [baz hrange₁]; simp
+          mexists c₁.val.length + c₂.val.length - (i₁ + 1) - i₂
+          mconstructor; · mpure_intro; trivial
+          mconstructor; · mpure_intro; grind
+          mconstructor; massumption; mpure_intro
+          constructor; · assumption
+          constructor; · exists hrange₂
+          cases result
+          case none => simp at hjoin ⊢; assumption
+          case some result => simp at hjoin ⊢; assumption
+  case pre => simp; mconstructor; massumption; mpure_intro; grind
+  case post.success r =>
+    simp; mrename_i h; mcases h with ⟨hstate, hresult⟩; rw [hresult]; simp
+    mconstructor; massumption; mpure_intro; trivial
+  case post.except => simp
+
+theorem joinPromotedTypesA_correct [Monad m] [MonadExcept String m] [Lean.Order.MonadTail m]
+    [WPMonad m ps] (c₁ c₂ : PromotionChain) :
+    ⦃stateIs s₀⦄ (joinPromotedTypesA c₁.val c₂.val : m _)
+    ⦃⇓ r => stateIs s₀ ∧ ⌜r = (c₁.join c₂).val⌝⦄ := by
+  unfold joinPromotedTypesA
+  apply WP_ite
+  case hifTrue =>
+    intro hempty₁; simp [hempty₁]; mintro hstate; mconstructor; massumption; mpure_intro; trivial
+  case hifFalse =>
+  intro hnotEmpty₁; apply WP_ite
+  case hifTrue =>
+    intro hempty₂; simp [hempty₂]; mintro hstate; mconstructor; massumption; mpure_intro; trivial
+  case hifFalse =>
+  intro hnotEmpty₂
+  apply WP_ite
+  case hifTrue =>
+    intro hc₁_longer; mintro hstate; simp; mspec joinPromotedTypesA'_correct
+    · grind
+    · order
+    · rename_i r; mrename_i h; mcases h with ⟨hstate, hresult⟩
+      mconstructor; massumption; mpure_intro
+      rw [join.commutative]; assumption
+  case hifFalse =>
+    intro hc₁_shorter; mintro hstate; simp; mspec joinPromotedTypesA'_correct
+    · grind
+    · order
+
+theorem AlgM.of_wp_run_eq
+    {α : Type}
+    {x : α} {prog : AlgM α} {fmA₀ fmA : FlowModelA}
+    (h : prog.run cfg fmA₀ = .ok (x, fmA)) (P : α → Prop) :
+    (⊢ₛ wp⟦prog⟧ (⇓? a => ⌜P a⌝)) → P x := by
+  intro hwp
+  apply ReaderT.of_wp_run (m := StateT FlowModelA (ExceptT String Id)) (ρ := Config) (prog := prog)
+    (r := cfg) P
+  case hcan =>
+    simp [MonadAttach.CanReturn, Id.run, StateT.run]
+    exists fmA₀, fmA
+  case hwp =>
+    have := hwp cfg
+    simp at this ⊢
+    assumption
+
+lemma wp_expand_readerT {prog : ReaderT ρ m α} [WP m ps] :
+    (wp⟦prog⟧ Q) r = wp⟦prog r⟧ (fun a => Q.fst a r, Q.snd) := by rfl
+
+lemma wp_expand_stateT {prog : StateT σ m α} [WP m ps] :
+    (wp⟦prog⟧ Q) s = wp⟦prog s⟧ (fun x => Q.fst x.fst x.snd, Q.snd) := by rfl
+
+lemma wp_expand_exceptT {prog : ExceptT ε m α} [WP m ps] :
+    wp⟦prog⟧ Q = wp⟦prog.run⟧ (fun x =>
+      match x with
+      | Except.ok a => Q.fst a
+      | Except.error e => Q.snd.fst e,
+      Q.snd.snd) := by
+  rewrite [WP.wp, ExceptT.instWP]
+  simp
+
+-- TODO: bad name?
+lemma wp_expand_id {α Q} {prog : Id α} :
+    wp⟦prog⟧ Q = wp⟦prog⟧ (PostCond.noThrow fun a => ⟨(Q.fst a).down⟩) := by rfl
+
+/--
+Given a WP characterization of an (AlgM α) program that is known not to raise errors, an input
+state, and a proof that the preconditions are satisfied, this theorem can be used to obtain:
+- The output of the program
+- The final state of the program
+- A proof that the postcondition holds for the given output and final state
+- A proof that the program, when run, actually produces the given output and final state.
+-/
+theorem AlgM.output_of_wp_run {P : Config → FlowModelA → ULift Prop}
+    {Q : α → Config → FlowModelA → ULift Prop} {prog : AlgM α}
+    (hwp : P ⊢ₛ wp⟦prog⟧ (.noThrow Q)) cfg fmA₀ :
+    (P cfg fmA₀).down → ∃ a fmA, (Q a cfg fmA).down ∧ prog cfg fmA₀ = .ok (a, fmA) := by
+  intro hpre
+  specialize hwp cfg fmA₀ hpre
+  simp [WP.wp, ReaderT.run, StateT.run, ExceptT.run, Id.run] at hwp
+  cases hok : prog cfg fmA₀ <;> simp [hok] at hwp
+  case ok r => exists r.fst, r.snd
+  case error e => simp [ExceptConds.false, ExceptConds.const] at hwp
+
+/--
+Given a WP characterization of an (AlgM α) program that might raise errors, an input state, a proof
+that the preconditions are satisfied, and a known output of the program, this theorem can be used to
+obtain a proof that the known output actually satisfies the postcondition.
+
+TODO: needed?
+-/
+theorem AlgM.post_of_wp_run {P : Config → FlowModelA → ULift Prop}
+    {Q : α → Config → FlowModelA → ULift Prop} {prog : AlgM α}
+    (hwp : P ⊢ₛ wp⟦prog⟧ (.mayThrow Q)) cfg fmA₀ :
+    (P cfg fmA₀).down → ∀ a fmA, prog cfg fmA₀ = .ok (a, fmA) → (Q a cfg fmA).down := by
+  intro hpre
+  specialize hwp cfg fmA₀ hpre
+  simp [WP.wp, ReaderT.run, StateT.run, ExceptT.run, Id.run] at hwp
+  cases hok : prog cfg fmA₀ <;> simp [hok] at hwp
+  case ok r =>
+    intro a' fmA' hok'
+    injection hok' with hok'; subst hok'
+    simp at hwp; assumption
+  case error e => intro a' fmA' hok'; contradiction
+
+theorem joinPromotedTypes_correct (c₁ c₂ : PromotionChain) :
+    (joinPromotedTypesA c₁.val c₂.val : ExceptT String Id _).run = .ok (c₁.join c₂).val := by
+  symm; apply ExceptT.of_wp_run (prog := (joinPromotedTypesA c₁.val c₂.val : ExceptT String Id _))
+  · simp [MonadAttach.CanReturn, Id.run]
+  · mspec joinPromotedTypesA_correct
+    rename_i r
+    mrename_i h
+    mcases h with ⟨hstate, hr⟩
+    mpure_intro
+    simp [hr]
+end
+
+theorem ValueModelA.refines.join {vmA₁ vmA₂ : ValueModelA}
+    {vm₁ vm₂ : ValueModel} :
+    vmA₁.refines vm₁ → vmA₂.refines vm₂ → (vmA₁.join vmA₂).refines (vm₁.join vm₂) := by
+  rintro hrefines₁ hrefines₂
+  simp [ValueModelA.join, ValueModel.join]
+  simp [hrefines₁.types, hrefines₂.types]
+  rw [joinPromotedTypes_correct vm₁.promotedTypes vm₂.promotedTypes]
+  constructor; simp
+
+inductive FlowModelA_refines_cases (fmA : FlowModelA)
+    (fm : FlowModel) (v : Variable) : Prop where
+  -- TODO: rename to "absent"?
+  | nones (hlookupA : fmA.env[v]? = none) (hlookup : fm.env v = none) :
+      FlowModelA_refines_cases fmA fm v
+  -- TODO: rename to "present"?
+  | somes
+        {vmA : ValueModelA} {vm : ValueModel} (hlookupA : fmA.env[v]? = some vmA)
+        (hlookup : fm.env v = some vm) (hrefines_vm : vmA.refines vm) :
+      FlowModelA_refines_cases fmA fm v
+
+structure FlowModelA.refines (fmA : FlowModelA)
+    (fm : FlowModel) : Prop where
+  lookup (v : Variable) : FlowModelA_refines_cases fmA fm v
+  -- TODO: needed?
+  --nones (v : Variable) : fmA.env[v]? = none ↔ fm.env v = none
+  --somes
+  --  {v : Variable} {vmA : ValueModelA} {vm : ValueModel}
+  --  (hsomeA : fmA.env[v]? = some vmA) (hsome : fm.env v = some vm) :
+  --  vmA.refines vm
+
+-- TODO: needed?
+--theorem FlowModelA.refines.mems
+--    {fmA : FlowModelA} {fm : FlowModel} (hrefines : fmA.refines fm) (v : Variable) :
+--    v ∈ fmA.env ↔ (fm.env v).isSome := by sorry
+
+-- TODO: needed?
+--theorem FlowModelA.refines.notMems
+--    {fmA : FlowModelA} {fm : FlowModel} (hrefines : fmA.refines fm) (v : Variable) :
+--    ¬v ∈ fmA.env ↔ fm.env v = none := by rw [←hrefines.nones v]; simp
+
+-- TODO: needed?
+--theorem FlowModelA.refines.eq_some_iff
+--    {fmA : FlowModelA} {fm : FlowModel} {vm : ValueModel} {v : Variable}
+--    (hrefines : fmA.refines fm) :
+--    fm.env v = some vm ↔ ∃ vmA : ValueModelA, fmA.env[v]? = some vmA ∧ vmA.refines vm := by
+--  constructor
+--  case mp =>
+--    intro hlookup
+--    cases hlookupA : fmA.env[v]? <;> simp
+--    case none => rw [hrefines.nones] at hlookupA; simp_all
+--    case some vmA => exact hrefines.somes hlookupA hlookup
+--  case mpr =>
+--    rintro ⟨vmA, hlookupA, hrefines_vm⟩
+--    cases hlookup : fm.env v <;> simp
+--    case none => rw [←hrefines.nones] at hlookup; simp_all
+--    case some vm' =>
+--      have hrefines_vm' : vmA.refines vm' := hrefines.somes hlookupA hlookup
+--      apply ValueModelA.refines.unique hrefines_vm' hrefines_vm
+
+theorem FlowModelA.refines.empty :
+    (.empty : FlowModelA).refines FlowModel.empty := by
+  constructor; intro v
+  apply FlowModelA_refines_cases.nones (by simp [FlowModelA.empty]) (by simp [FlowModel.empty])
+
+theorem FlowModelA.refines.isEmpty {fmA : FlowModelA} {fm : FlowModel}
+    (hrefines : fmA.refines fm) :
+    fmA.env.isEmpty ↔ ∀ v, fm.env v = none := by
+  constructor
+  case mp =>
+    intro hemptyA v
+    have : fmA.env[v]? = none := by exact Std.HashMap.getElem?_of_isEmpty hemptyA
+    cases hrefines.lookup v <;> simp_all
+  case mpr =>
+    intro hempty
+    rw [Std.HashMap.isEmpty_iff_forall_not_mem]
+    intro v
+    cases hrefines.lookup v <;> simp_all
+
+@[simp]
+theorem FlowModelA.refines.isEmpty_simp {fmA : FlowModelA} :
+    fmA.env.isEmpty → fmA.refines ⟨fun _ => none⟩ := by
+  intro hempty
+  constructor; intro v
+  apply FlowModelA_refines_cases.nones (Std.HashMap.getElem?_of_isEmpty hempty) (by simp)
+
+lemma FlowModelA.refines.some_if_some {fmA : FlowModelA}
+    {fm₁ fm₂ : FlowModel} {v vm} :
+    fmA.refines fm₁ → fmA.refines fm₂ → fm₁.env v = some vm → fm₂.env v = some vm := by
+  intro hrefines₁ hrefines₂ hlookup₁
+  cases hrefines₁.lookup v <;> simp_all; subst_eqs
+  case somes vmA₁ hlookupA₁ hlookup₁' hrefines_vm₁ =>
+    cases hrefines₂.lookup v <;> simp_all; subst_eqs
+    case somes vm₂ hlookupA₂ hlookup₂ hrefines_vm₂ =>
+      exact ValueModelA.refines.unique hrefines_vm₂ hrefines_vm₁
+
+-- TODO: needed?
+theorem FlowModelA.refines.unique {fmA : FlowModelA} {fm₁ fm₂ : FlowModel} :
+    fmA.refines fm₁ → fmA.refines fm₂ → fm₁ = fm₂ := by
+  intro hrefines₁ hrefines₂
+  ext; rename_i v vm
+  constructor <;> apply some_if_some (by assumption) (by assumption)
+
+@[simp]
+theorem FlowModelA.refines.insert {fmA : FlowModelA} {fm : FlowModel}
+    {vmA : ValueModelA} {vm : ValueModel} (v : Variable) :
+    fmA.refines fm → vmA.refines vm →
+    (FlowModelA.mk (fmA.env.insert v vmA)).refines (fm.set v vm) := by
+  intro hrefines_fm hrefines_vm; constructor; intro v'
+  by_cases heq : v = v' <;> subst_eqs
+  case pos =>
+    apply FlowModelA_refines_cases.somes (by simp; rfl) (by simp; rfl) (by assumption)
+  case neg =>
+    cases hrefines_fm.lookup v'
+    case nones hlookupA hlookup =>
+      apply FlowModelA_refines_cases.nones (by simp_all) (by simp_all)
+    case somes vmA' vm' hlookupA hlookup hrefines_vm' =>
+      apply FlowModelA_refines_cases.somes
+        (by simp_all [Std.HashMap.getElem?_insert]; rfl) (by simp_all; rfl) (by assumption)
+
+theorem FlowModelA.refines.tryPromote
+    {fmA : FlowModelA} {fm : FlowModel} (hrefines : fmA.refines fm) ref? T :
+    ∃ fmA', tryPromoteA ref? T cfg fmA = Except.ok ((), fmA') ∧
+    fmA'.refines (fm.tryPromote ref? T) := by
+  simp [tryPromoteA, FlowModel.tryPromote]
+  cases ref? <;> simp_all [AlgM_pure_eq, AlgM_bind_eq]
+  case none => exists fmA
+  case some ref =>
+    cases ref; simp_all
+    case var v =>
+      cases hrefines.lookup v <;> simp_all [AlgM_get_eq, AlgM_pure_eq]
+      case nones => exists fmA
+      case somes vmA vm hlookupA hlookup hrefines_vm =>
+        rw [hrefines_vm.currentTypes]
+        by_cases hT_lt_current : T < vm.currentType v.type <;>
+          simp_all [AlgM_pure_eq, AlgM_modify_eq]
+        case neg => exists fmA
+        case pos =>
+          exists ⟨fmA.env.insert v ⟨[T]⟩⟩
+          simp
+          apply FlowModelA.refines.insert v hrefines
+          simp
+
+-- TODO: needed?
+section
+variable {α β : Type} [BEq α] [LawfulBEq α] [Hashable α] [LawfulHashable α]
+variable {f : β → β → β} {m₁ m₂ : Std.HashMap α β}
+
+theorem mergeMaps_none₁ {k : α} : k ∉ m₁ → k ∉ mergeMaps f m₁ m₂ := by
+  simp_all [mergeMaps, Std.HashMap.mem_filterMap]
+
+theorem mergeMaps_none₂ {k : α} : k ∉ m₂ → k ∉ mergeMaps f m₁ m₂ := by
+  simp_all [mergeMaps, Std.HashMap.mem_filterMap]
+
+theorem mergeMaps_some {k : α} {v₁ v₂ : β} :
+    m₁[k]? = some v₁ → m₂[k]? = some v₂ → (mergeMaps f m₁ m₂)[k]? = f v₁ v₂ := by
+  simp_all [mergeMaps]
+
+end
+
+theorem FlowModelA.refines.join {fmA₁ fmA₂ : FlowModelA}
+    {fm₁ fm₂ : FlowModel} :
+    fmA₁.refines fm₁ → fmA₂.refines fm₂ → (fmA₁.join fmA₂).refines (fm₁.join fm₂) := by
+  intro hrefines₁ hrefines₂
+  simp [FlowModelA.join, FlowModel.join]
+  by_cases_iff hrefines₁.isEmpty <;> simp_all
+  case neg hnonEmpty₁ hnonEmptyA₁ =>
+    by_cases_iff hrefines₂.isEmpty <;> simp_all
+    case pos => (conv => enter [2, 1, v]; tactic => split); simp_all
+    case neg hnonEmpty₂ hnonEmptyA₂ =>
+      constructor; intro v
+      cases hrefines₁.lookup v
+      case nones hlookupA₁ hlookup₁ =>
+        apply FlowModelA_refines_cases.nones (by simp_all [mergeMaps_none₁]) (by simp_all)
+      case somes vmA₁ vm₁ hlookupA₁ hlookup₁ hrefines_vm₁ =>
+        cases hrefines₂.lookup v
+        case nones hlookupA₂ hlookup₂ =>
+          apply FlowModelA_refines_cases.nones (by simp_all [mergeMaps_none₂]) (by simp_all)
+        case somes vmA₂ vm₂ hlookupA₂ hlookup₂ hrefines_vm₂ =>
+          apply FlowModelA_refines_cases.somes
+            (by simp_all [mergeMaps_some]; rfl)
+            (by simp_all; rfl)
+            (by simp_all [hrefines_vm₁.join hrefines_vm₂])
+
+structure ExprModelA.refines (emA : ExprModelA)
+    (fmA : FlowModelA) (em : ExprModel) :
+    Prop where
+  types : emA.type = em.type
+  ref?s : emA.ref? = em.ref?
+  fm_trues : (emA.boolInfo.getD (fmA, fmA)).fst.refines em.fm_true
+  fm_falses : (emA.boolInfo.getD (fmA, fmA)).snd.refines em.fm_false
+
+theorem ExprModelA.refines.noBoolInfo {fmA fm} (hrefines : fmA.refines fm) T ref? :
+    (⟨T, ref?, none⟩ : ExprModelA).refines fmA ⟨T, ref?, fm, fm⟩ := by
+  constructor <;> simp_all
+
+-- TODO: needed?
+--theorem exprModelA_boolInfo_getD_sound {emA fmA fmA_true fmA_false} :
+--    (emA : ExprModelA).boolInfo.getD (fmA, fmA) = (fmA_true, fmA_false) →
+--    emA.interp fmA = ⟨emA.type, emA.ref?, fmA_true.interp, fmA_false.interp⟩ := by
+--  intro h
+--  simp [ExprModelA.interp]
+--  simp [Option.getD] at h
+--  cases hboolInfo : emA.boolInfo <;> simp [hboolInfo] at h <;> clear hboolInfo
+--  case none =>
+--    rcases h with ⟨rfl, rfl⟩ ; simp
+--  case some boolInfo =>
+--    subst h; simp
+
+-- TODO: needed?
+@[simp]
+theorem ExprModelA.refines.fm_eq_afters_if_noBoolInfo {emA : ExprModelA} {fmA}
+    {em : ExprModel} (hboolInfo : emA.boolInfo = none) :
+    emA.refines fmA em → em.fm_after = em.fm_true ∧ em.fm_true = em.fm_false := by
+  intro hrefines_em
+  have hrefines_fm_true := hrefines_em.fm_trues; simp [hboolInfo] at hrefines_fm_true
+  have hrefines_fm_false := hrefines_em.fm_falses; simp [hboolInfo] at hrefines_fm_false
+  have hfm_true_eq_false := hrefines_fm_true.unique hrefines_fm_false
+  simp [ExprModel.fm_after, hfm_true_eq_false]
+
+-- TODO: needed?
+--@[simp]
+--theorem ExprModelA.refines.refines_fm_true_eq_false_eq_after_if_noBoolInfo
+--    {emA : ExprModelA} {fmA em} (hboolInfo : emA.boolInfo = none) :
+--    emA.refines fmA em →
+--    em.fm_true = em.fm_false ∧ em.fm_false = em.fm_after := by sorry
+
+-- TODO: trying to fold this into elabExprA_correct
+--theorem elabExprA.consistent_emA_fmA {e fmA₀ m emA fmA em} :
+--    elabExprA e fmA₀ = Except.ok ((m, emA), fmA) → emA.refines fmA em →
+--    fmA.refines em.fm_after := by
+--  intro hok hrefines_em
+--  cases e <;> simp [elabExprA] at hok
+--  case var v =>
+--    cases hlookup : fmA₀.env[v]? <;> simp [hlookup] at hok
+--    case some vmA =>
+--      rcases hok with ⟨⟨rfl, rfl⟩, rfl⟩
+--      exact hrefines_em.refines_fm_after_if_noBoolInfo rfl
+--  case nullCheck e₁ =>
+--    cases hok₁ : elabExprA e₁ fmA₀ <;> simp [hok₁] at hok
+--    rename_i this; rcases this with ⟨⟨m₁, emA₁⟩, fmA₁⟩; simp at hok
+--    cases htryPromote : tryPromoteA emA₁.ref? emA₁.type.nonNull fmA₁ <;> simp [htryPromote] at hok
+--    rename_i this; rcases this with ⟨_, fmA'⟩; simp at hok
+--    rcases hok with ⟨⟨rfl, rfl⟩, rfl⟩
+--    exact hrefines_em.refines_fm_after_if_noBoolInfo rfl
+--  case as e₁ T =>
+--    cases hok₁ : elabExprA e₁ fmA₀ <;> simp [hok₁] at hok
+--    rename_i this; rcases this with ⟨⟨m₁, emA₁⟩, fmA₁⟩; simp at hok
+--    cases htryPromote : tryPromoteA emA₁.ref? T fmA₁ <;> simp [htryPromote] at hok
+--    rename_i this; rcases this with ⟨_, fmA'⟩; simp at hok
+--    rcases hok with ⟨⟨rfl, rfl⟩, rfl⟩
+--    exact hrefines_em.refines_fm_after_if_noBoolInfo rfl
+--  case null =>
+--    rcases hok with ⟨⟨rfl, rfl⟩, rfl⟩
+--    exact hrefines_em.refines_fm_after_if_noBoolInfo rfl
+
+structure elabExprA.Correctness (e : Expr) : Prop where
+  complete : ∀ {fm₀ m em} {fmA₀ : FlowModelA}, fmA₀.refines fm₀ →
+    ElabExpr fm₀ e m em → ∃ fmA emA,
+      elabExprA e cfg fmA₀ = Except.ok ((m, emA), fmA) ∧
+      fmA.refines em.fm_after ∧ emA.refines fmA em
+  sound : ∀ {fm₀ m emA fmA} {fmA₀ : FlowModelA}, fmA₀.refines fm₀ →
+      elabExprA e cfg fmA₀ = Except.ok ((m, emA), fmA) → ∃ em,
+      ElabExpr fm₀ e m em ∧ fmA.refines em.fm_after ∧ emA.refines fmA em
+
+theorem elabExprA.correct.var (v : Variable) :
+    elabExprA.Correctness (cfg := cfg) (.var v : Expr) := by
+  constructor
+  case complete =>
+    intro fm₀ m em fmA₀ hrefines_fm₀ helab; simp [elabExprA, AlgM_get_eq, AlgM_bind_eq]
+    cases helab; case var vm T hlookup hcurrentType =>
+      cases hrefines_fm₀.lookup v <;> simp_all [AlgM_pure_eq]; subst_eqs
+      case somes vmA hlookupA hlookup hrefines_vm =>
+        simp [hrefines_vm.currentTypes]
+        refine ⟨?_, ?_, ?_, ?_, ?_⟩; rotate_left 2
+        · congr; rfl; rfl
+        · assumption
+        · constructor <;> simp <;> assumption
+  case sound =>
+    intro fm₀ m emA fmA fmA₀ hrefines_fm₀ hok; simp [elabExprA, AlgM_bind_eq] at hok
+    cases hrefines_fm₀.lookup v <;> simp_all [AlgM_get_eq, AlgM_throw_eq_ok_contra]
+    case somes vmA vm hlookupA hlookup hrefines_vm =>
+      simp_all [hrefines_vm.currentTypes]
+      rcases hok with ⟨⟨rfl, rfl⟩, rfl⟩
+      exists ⟨vm.currentType v.type, some (.var v), fm₀, fm₀⟩; simp_all
+      constructor
+      · exact ElabExpr.var hlookup rfl
+      · exact ExprModelA.refines.noBoolInfo
+          hrefines_fm₀ (vm.currentType v.type) (some (Reference.var v))
+
+theorem elabExprA.correct.nullCheck (e₁ : Expr) (hcorrect₁ :
+    elabExprA.Correctness (cfg := cfg) e₁) :
+    elabExprA.Correctness (cfg := cfg) e₁.nullCheck := by
+  constructor
+  case complete =>
+    intro fm₀ m em fmA₀ hrefines_fm₀ helab; simp [elabExprA, AlgM_bind_eq, AlgM_map_eq]
+    cases helab; case nullCheck m₁ em₁ fm htryPromote helab₁ =>
+      rcases em₁ with ⟨T₁, ref?₁, fm_true₁, fm_false₁⟩; simp_all
+      obtain ⟨fmA₁, ⟨T₁', ref?₁', boolInfo₁⟩, hok₁, hrefines_fm₁, hrefines_em₁⟩ :=
+        hcorrect₁.complete hrefines_fm₀ helab₁; simp_all
+      rcases hrefines_em₁.types with rfl; simp_all
+      rcases hrefines_em₁.ref?s with rfl; simp_all
+      obtain ⟨fmA, hok_tryPromote, hrefines_fmA⟩ :=
+        hrefines_fm₁.tryPromote (cfg := cfg) ref?₁' (NonNull T₁'); simp_all
+      refine ⟨?_, ?_, ?_, ?_, ?_⟩; rotate_left 2
+      · congr; rfl; rfl
+      · assumption
+      · constructor <;> simp <;> assumption
+  case sound =>
+    intro fm₀ m emA fmA fmA₀ hrefines_fm₀ hok; simp [elabExprA, AlgM_bind_eq, AlgM_map_eq] at hok
+    cases hok₁ : elabExprA e₁ cfg fmA₀ <;> simp_all
+    case ok result₁ =>
+      rcases result₁ with ⟨⟨m₁, ⟨T₁, ref?₁, boolInfo₁⟩⟩, fmA₁⟩; simp_all
+      rcases hcorrect₁.sound hrefines_fm₀ hok₁ with ⟨em₁, helab₁, hrefines_fm₁, hrefines_em₁⟩
+      generalize hfm₁ : em₁.fm_after = fm₁; simp_all
+      rcases em₁ with ⟨T₁', ref?₁', fm_true₁, fm_false₁⟩
+      rcases hrefines_em₁.types with rfl; simp_all
+      rcases hrefines_em₁.ref?s with rfl; simp_all
+      obtain ⟨fmA', hok_tryPromote, hrefines_fmA'⟩ :=
+        hrefines_fm₁.tryPromote (cfg := cfg) ref?₁ (NonNull T₁); simp_all
+      generalize hfm : (FlowModel.tryPromote ref?₁ (NonNull T₁) fm₁) = fm; simp_all
+      generalize hem : (⟨NonNull T₁, none, fm, fm⟩ : ExprModel) = em
+      injections; subst fmA m emA
+      have hrefines_em := ExprModelA.refines.noBoolInfo hrefines_fmA' (NonNull T₁) none;
+        rw [hem] at hrefines_em
+      exists em
+      refine ⟨?_, ?_, ?_⟩
+      · subst hem; apply ElabExpr.nullCheck helab₁ (by simp_all)
+      · subst hem; simp [ExprModel.fm_after]; assumption
+      · assumption
+
+theorem elabExprA.correct.asExpr (e₁ : Expr) T
+    (hcorrect₁ : elabExprA.Correctness (cfg := cfg) e₁) :
+    elabExprA.Correctness (cfg := cfg) (e₁.as T) := by
+  constructor
+  case complete =>
+    intro fmA₀ fm₀ m em hrefines_fm₀ helab; simp [elabExprA, AlgM_bind_eq, AlgM_map_eq]
+    cases helab; case asExpr m₁ em₁ fm helab₁ htryPromote =>
+      rcases em₁ with ⟨T₁, ref?₁, fm_true₁, fm_false₁⟩; simp_all
+      obtain ⟨fmA₁, ⟨T₁', ref?₁', boolInfo₁⟩, hok₁, hrefines_fm₁, hrefines_em₁⟩ :=
+        hcorrect₁.complete hrefines_fm₀ helab₁; simp_all
+      rcases hrefines_em₁.types with rfl; simp_all
+      rcases hrefines_em₁.ref?s with rfl; simp_all
+      obtain ⟨fmA, hok_tryPromote, hrefines_fmA⟩ :=
+        hrefines_fm₁.tryPromote (cfg := cfg) ref?₁' T; simp_all
+      refine ⟨?_, ?_, ?_, ?_, ?_⟩; rotate_left 2
+      · congr; rfl; rfl
+      · assumption
+      · constructor <;> simp <;> assumption
+  case sound =>
+    intro fm₀ m emA fmA fmA₀ hrefines_fm₀ hok; simp [elabExprA, AlgM_bind_eq, AlgM_map_eq] at hok
+    cases hok₁ : elabExprA e₁ cfg fmA₀ <;> simp_all
+    case ok result₁ =>
+      rcases result₁ with ⟨⟨m₁, ⟨T₁, ref?₁, boolInfo₁⟩⟩, fmA₁⟩; simp_all
+      rcases hcorrect₁.sound hrefines_fm₀ hok₁ with ⟨em₁, helab₁, hrefines_fm₁, hrefines_em₁⟩
+      generalize hfm₁ : em₁.fm_after = fm₁; simp_all
+      rcases em₁ with ⟨T₁', ref?₁', fm_true₁, fm_false₁⟩
+      rcases hrefines_em₁.types with rfl; simp_all
+      rcases hrefines_em₁.ref?s with rfl; simp_all
+      obtain ⟨fmA', hok_tryPromote, hrefines_fmA'⟩ :=
+        hrefines_fm₁.tryPromote (cfg := cfg) ref?₁ T; simp_all
+      generalize hfm : (FlowModel.tryPromote ref?₁ T fm₁) = fm; simp_all
+      generalize hem : (⟨T, none, fm, fm⟩ : ExprModel) = em
+      injections; subst fmA' m emA
+      have hrefines_em := ExprModelA.refines.noBoolInfo hrefines_fmA' T none;
+        rw [hem] at hrefines_em
+      exists em
+      refine ⟨?_, ?_, ?_⟩
+      · subst hem; apply ElabExpr.asExpr helab₁ (by simp_all)
+      · subst hem; simp [ExprModel.fm_after]; assumption
+      · assumption
+
+theorem elabExprA.correct.nullLiteral :
+    elabExprA.Correctness (cfg := cfg) (.null : Expr) := by
+  constructor
+  case complete =>
+    intro fmA₀ fm₀ m em hrefines_fm₀ helab; simp [elabExprA, AlgM_pure_eq]
+    cases helab; simp; case nullLiteral =>
+      refine ⟨?_, ?_, ?_, ?_, ?_⟩; rotate_left 2
+      · congr; rfl; rfl
+      · assumption
+      · constructor <;> simp <;> assumption
+  case sound =>
+    intro fm₀ m emA fmA fmA₀ hrefines_fm₀ hok; simp [elabExprA] at hok
+    rcases hok with ⟨⟨rfl, rfl⟩, rfl⟩
+    exists ⟨Γ.Null, none, fm₀, fm₀⟩; simp_all
+    constructor
+    · apply ElabExpr.nullLiteral
+    · exact ExprModelA.refines.noBoolInfo hrefines_fm₀ Γ.Null none
+
+theorem elabExprA.correct (e : Expr) :
+    elabExprA.Correctness (cfg := cfg) e := by
+  constructor
+  case complete =>
+    intro fmA₀ fm₀ m em hrefines_fm₀ helab
+    cases h : e <;> rw [h] at helab
+    case var v => apply (elabExprA.correct.var v).complete hrefines_fm₀ helab
+    case nullCheck e₁ =>
+      apply (elabExprA.correct.nullCheck e₁ (elabExprA.correct e₁)).complete hrefines_fm₀ helab
+    case as e₁ T =>
+      apply (elabExprA.correct.asExpr e₁ T (elabExprA.correct e₁)).complete hrefines_fm₀ helab
+    case null => apply elabExprA.correct.nullLiteral.complete hrefines_fm₀ helab
+  case sound =>
+    intro fm₀ m emA fmA fmA₀ hrefines_fm₀ hok
+    cases h : e <;> rw [h] at hok
+    case var v => apply (elabExprA.correct.var v).sound hrefines_fm₀ hok
+    case nullCheck e₁ =>
+      apply (elabExprA.correct.nullCheck e₁ (elabExprA.correct e₁)).sound hrefines_fm₀ hok
+    case as e₁ T =>
+      apply (elabExprA.correct.asExpr e₁ T (elabExprA.correct e₁)).sound hrefines_fm₀ hok
+    case null => apply elabExprA.correct.nullLiteral.sound hrefines_fm₀ hok
+
+structure elabStmtA.Correctness (s : Stmt) : Prop where
+  complete :
+    ∀ {fm₀ m fm} {fmA₀ : FlowModelA}, fmA₀.refines fm₀ →
+      ElabStmt fm₀ s m fm →
+      ∃ fmA, elabStmtA s cfg fmA₀ = Except.ok (m, fmA) ∧ fmA.refines fm
+  sound :
+    ∀ {fm₀ m fmA} {fmA₀ : FlowModelA},
+      fmA₀.refines fm₀ → elabStmtA s cfg fmA₀ = Except.ok (m, fmA) →
+      ∃ fm, ElabStmt fm₀ s m fm ∧ fmA.refines fm
+
+structure elabStmtsA.Correctness (ss : List Stmt) : Prop where
+  complete :
+    ∀ {fm₀ m fm} {fmA₀ : FlowModelA}, fmA₀.refines fm₀ →
+      ElabStmts fm₀ ss m fm →
+      ∃ fmA, elabStmtsA ss cfg fmA₀ = Except.ok (m, fmA) ∧ fmA.refines fm
+  sound :
+    ∀ {fm₀ m fmA} {fmA₀ : FlowModelA},
+      fmA₀.refines fm₀ → elabStmtsA ss cfg fmA₀ = Except.ok (m, fmA) →
+      ∃ fm, ElabStmts fm₀ ss m fm ∧ fmA.refines fm
+
+theorem elabStmtA.correct.declare (n : String) (T : τ) :
+    elabStmtA.Correctness (cfg := cfg) (.declare n T) := by
+  constructor
+  case complete =>
+    intro fm₀ m fm fmA₀ hrefines_fm₀ helab; simp [elabStmtA, AlgM_map_eq, AlgM_modify_eq]
+    cases helab; case declare =>
+      refine ⟨?_, ?_, ?_⟩; rotate_left
+      · congr; rfl
+      · apply hrefines_fm₀.insert ⟨n, T⟩ (by simp)
+  case sound =>
+    intro fm₀ m fmA fmA₀ hrefines_fm₀ hok; simp [elabStmtA] at hok
+    rcases hok with ⟨rfl, rfl⟩
+    exists fm₀.set ⟨n, T⟩ ⟨∅⟩
+    constructor
+    · apply ElabStmt.declare fm₀ n T
+    · apply hrefines_fm₀.insert ⟨n, T⟩ ValueModelA.refines.empty
+
+theorem elabStmtA.correct.exprStmt
+    (e₁ : Expr) (hcorrect₁ : elabExprA.Correctness (cfg := cfg) e₁) :
+    elabStmtA.Correctness (cfg := cfg) (.exprStmt e₁) := by
+  constructor
+  case complete =>
+    intro fm₀ m fm fmA₀ hrefines_fm₀ helab; simp [elabStmtA, AlgM_map_eq]
+    cases helab; case exprStmt em₁ helab₁ =>
+      rcases em₁ with ⟨T₁, ref?₁, fm_true₁, fm_false₁⟩
+      obtain ⟨fmA₁, ⟨T₁', ref?₁', boolInfo₁⟩, hok₁, hrefines_fm₁, hrefines_em₁⟩ :=
+        hcorrect₁.complete hrefines_fm₀ helab₁; simp_all
+      refine ⟨?_, ?_, ?_⟩; rotate_left
+      · congr; rfl
+      · assumption
+  case sound =>
+    intro fm₀ m fmA fmA₀ hrefines_fm₀ hok; simp [elabStmtA, AlgM_map_eq] at hok
+    cases hok₁ : elabExprA e₁ cfg fmA₀ <;> simp_all; case ok result₁ =>
+    injections; subst m fmA
+    rcases result₁ with ⟨⟨m₁, emA₁⟩, fmA₁⟩; simp_all
+    rcases hcorrect₁.sound hrefines_fm₀ hok₁ with ⟨em₁, helab₁, hrefines_fm₁, hrefines_em₁⟩
+    exists em₁.fm_after; simp_all
+    exact ElabStmt.exprStmt helab₁
+
+theorem elabStmtA.correct.ifStmt
+    (e₁ : Expr) (s₂ s₃ : Stmt)
+    (hcorrect₁ : elabExprA.Correctness (cfg := cfg) e₁)
+    (hcorrect₂ : elabStmtA.Correctness (cfg := cfg) s₂)
+    (hcorrect₃ : elabStmtA.Correctness (cfg := cfg) s₃) :
+    elabStmtA.Correctness (cfg := cfg) (.ifStmt e₁ s₂ s₃) := by
+  constructor
+  case complete =>
+    intro fm₀ m em fmA₀ hrefines_fm₀ helab; simp [elabStmtA, AlgM_bind_eq]
+    cases helab; case ifStmt m₁ em₁ m₂ fm₂ m₃ fm₃ his_bool helab₁ helab₂ helab₃ =>
+      rcases em₁ with ⟨T₁, ref?₁, fm_true₁, fm_false₁⟩; simp_all
+      obtain ⟨fmA₁, ⟨T₁', ref?₁', boolInfo₁⟩, hok₁, hrefines_fm₁, hrefines_em₁⟩ :=
+        hcorrect₁.complete hrefines_fm₀ helab₁
+      rcases hrefines_em₁.types with rfl; simp_all [AlgM_bind_eq, AlgM_map_eq, AlgM_set_eq]
+      rcases hrefines_em₁.ref?s with rfl; simp_all
+      obtain hrefines_fm₁_true := hrefines_em₁.fm_trues; simp_all
+      obtain ⟨fmA₂, hok₂, hrefines_fm₂⟩ := hcorrect₂.complete hrefines_fm₁_true helab₂;
+        simp_all [AlgM_get_eq]
+      obtain hrefines_fm₁_false := hrefines_em₁.fm_falses; simp_all
+      obtain ⟨fmA₃, hok₃, hrefines_fm₃⟩ := hcorrect₃.complete hrefines_fm₁_false helab₃; simp_all
+      refine ⟨?_, ?_, ?_⟩; rotate_left
+      · congr; rfl
+      · exact FlowModelA.refines.join hrefines_fm₂ hrefines_fm₃
+  case sound =>
+    intro fm₀ m fmA fmA₀ hrefines_fm₀ hok; simp [elabStmtA, AlgM_bind_eq] at hok
+    cases hok₁ : elabExprA e₁ cfg fmA₀ <;> simp_all; case ok result₁ =>
+    rcases result₁ with ⟨⟨m₁, emA₁⟩, fmA₁⟩; simp_all
+    rcases hcorrect₁.sound hrefines_fm₀ hok₁ with ⟨em₁, helab₁, hrefines_fm₁, hrefines_em₁⟩
+    rcases emA₁ with ⟨T₁, ref?₁, boolInfo₁⟩
+    rcases hrefines_em₁.types with rfl; simp_all
+    by_cases his_bool : em₁.type = Γ.bool <;>
+      simp_all [AlgM_bind_eq, AlgM_set_eq, AlgM_throw_eq_ok_contra];
+      case pos =>
+    cases hok₂ : elabStmtA s₂ cfg (boolInfo₁.getD (fmA₁, fmA₁)).fst <;> simp_all [AlgM_get_eq];
+      case ok result₂ =>
+    rcases result₂ with ⟨m₂, fmA₂⟩; simp_all
+    rcases hcorrect₂.sound hrefines_em₁.fm_trues hok₂ with ⟨fm₂, helab₂, hrefines_fm₂⟩
+    cases hok₃ : elabStmtA s₃ cfg (boolInfo₁.getD (fmA₁, fmA₁)).snd <;> simp_all; case ok result₃ =>
+    rcases result₃ with ⟨m₃, fmA₃⟩; simp_all
+    rcases hcorrect₃.sound hrefines_em₁.fm_falses hok₃ with ⟨fm₃, helab₃, hrefines_fm₃⟩
+    rcases hok with ⟨rfl, rfl⟩
+    exists fm₂.join fm₃
+    constructor
+    · apply ElabStmt.ifStmt helab₁ his_bool helab₂ helab₃
+    · exact FlowModelA.refines.join hrefines_fm₂ hrefines_fm₃
+
+theorem elabStmtA.correct.block
+    (ss₁ : List Stmt) (hcorrect₁ : elabStmtsA.Correctness (cfg := cfg) ss₁) :
+    elabStmtA.Correctness (cfg := cfg) (.block ss₁) := by
+  constructor
+  case complete =>
+    intro fm₀ m fm fmA₀ hrefines_fm₀ helab; simp [elabStmtA, AlgM_map_eq]
+    cases helab; case block ms₁ helab₁ =>
+    obtain ⟨fmA₁, hok₁, hrefines_fm₁⟩ := hcorrect₁.complete hrefines_fm₀ helab₁; simp_all
+    refine ⟨?_, ?_, ?_⟩; rotate_left
+    · congr; rfl
+    · assumption
+  case sound =>
+    intro fm₀ m fmA fmA₀ hrefines_fm₀ hok; simp [elabStmtA, AlgM_map_eq] at hok
+    cases hok₁ : elabStmtsA ss₁ cfg fmA₀ <;> simp_all; case ok result₁ =>
+    rcases result₁ with ⟨m₁, fmA₂⟩; simp_all
+    rcases hcorrect₁.sound hrefines_fm₀ hok₁ with ⟨fm₁, helab₁, hrefines_fm₁⟩
+    rcases hok with ⟨rfl, rfl⟩
+    exists fm₁; simp_all
+    exact ElabStmt.block helab₁
+
+theorem elabStmtsA.correct.nil : elabStmtsA.Correctness (cfg := cfg) ([] : List Stmt) := by
+  constructor
+  case complete =>
+    intro fm₀ m fm fmA₀ hrefines_fm₀ helab; simp [elabStmtsA]
+    cases helab; case nil =>
+      exists fmA₀
+  case sound =>
+    intro fm₀ m fmA fmA₀ hrefines_fm₀ hok; simp [elabStmtsA] at hok
+    rcases hok with ⟨rfl, rfl⟩
+    exists fm₀; simp_all
+    exact ElabStmts.nil
+
+theorem elabStmtsA.correct.cons
+    (s₁ : Stmt) (ss₂ : List Stmt)
+    (hcorrect₁ : elabStmtA.Correctness (cfg := cfg) s₁)
+    (hcorrect₂ : elabStmtsA.Correctness (cfg := cfg) ss₂) :
+    elabStmtsA.Correctness (cfg := cfg) (s₁ :: ss₂) := by
+  constructor
+  case complete =>
+    intro fm₀ m fm fmA₀ hrefines_fm₀ helab; simp [elabStmtsA, AlgM_bind_eq, AlgM_map_eq]
+    cases helab; case cons fm₁ m₁ ms₂ helab₁ helab₂ =>
+      obtain ⟨fmA₁, hok₁, hrefines_fm₁⟩ := hcorrect₁.complete hrefines_fm₀ helab₁; simp_all
+      obtain ⟨fmA₂, hok₂, hrefines_fm₂⟩ := hcorrect₂.complete hrefines_fm₁ helab₂; simp_all
+      refine ⟨?_, ?_, ?_⟩; rotate_left
+      · congr; rfl
+      · assumption
+  case sound =>
+    intro fm₀ m fmA fmA₀ hrefines_fm₀ hok; simp [elabStmtsA, AlgM_bind_eq, AlgM_map_eq] at hok
+    cases hok₁ : elabStmtA s₁ cfg fmA₀ <;> simp_all; case ok result₁ =>
+    rcases result₁ with ⟨m₁, fmA₁⟩; simp_all
+    rcases hcorrect₁.sound hrefines_fm₀ hok₁ with ⟨fm₁, helab₁, hrefines_fm₁⟩
+    cases hok₂ : elabStmtsA ss₂ cfg fmA₁ <;> simp_all; case ok result₂ =>
+    rcases result₂ with ⟨m₂, fmA₂⟩; simp_all
+    rcases hcorrect₂.sound hrefines_fm₁ hok₂ with ⟨fm₂, helab₂, hrefines_fm₂⟩
+    rcases hok with ⟨rfl, rfl⟩
+    exists fm₂; simp_all
+    apply ElabStmts.cons helab₁ helab₂
+
+mutual
+theorem elabStmtA.correct (s : Stmt) :
+    elabStmtA.Correctness (cfg := cfg) s := by
+  constructor
+  case complete =>
+    intro fm₀ m fm fmA₀ hrefines_fm₀ helab
+    cases h : s <;> rw [h] at helab
+    case declare n T => apply (elabStmtA.correct.declare n T).complete hrefines_fm₀ helab
+    case exprStmt e₁ =>
+      apply (elabStmtA.correct.exprStmt e₁ (elabExprA.correct e₁)).complete hrefines_fm₀ helab
+    case ifStmt e₁ s₂ s₃ =>
+      apply
+        (elabStmtA.correct.ifStmt
+            e₁ s₂ s₃ (elabExprA.correct e₁) (elabStmtA.correct s₂) (elabStmtA.correct s₃)).complete
+          hrefines_fm₀ helab
+    case block ss =>
+      apply (elabStmtA.correct.block ss (elabStmtsA.correct ss)).complete hrefines_fm₀ helab
+  case sound =>
+    intro fm₀ m fmA fmA₀ hrefines_fm₀ hok
+    cases h : s <;> rw [h] at hok
+    case declare n T => apply (elabStmtA.correct.declare n T).sound hrefines_fm₀ hok
+    case exprStmt e₁ =>
+      apply (elabStmtA.correct.exprStmt e₁ (elabExprA.correct e₁)).sound hrefines_fm₀ hok
+    case ifStmt e₁ s₂ s₃ =>
+      apply
+        (elabStmtA.correct.ifStmt
+            e₁ s₂ s₃ (elabExprA.correct e₁) (elabStmtA.correct s₂) (elabStmtA.correct s₃)).sound
+          hrefines_fm₀ hok
+    case block ss =>
+      apply (elabStmtA.correct.block ss (elabStmtsA.correct ss)).sound hrefines_fm₀ hok
+
+theorem elabStmtsA.correct (ss : List Stmt) :
+    elabStmtsA.Correctness (cfg := cfg) ss := by
+  constructor
+  case complete =>
+    intro fm₀ m fm fmA₀ hrefines_fm₀ helab
+    cases h : ss <;> rw [h] at helab
+    case nil => apply elabStmtsA.correct.nil.complete hrefines_fm₀ helab
+    case cons s ss =>
+      apply (elabStmtsA.correct.cons s ss (elabStmtA.correct s) (elabStmtsA.correct ss)).complete
+        hrefines_fm₀ helab
+  case sound =>
+    intro fm₀ m fmA fmA₀ hrefines_fm₀ hok
+    cases h : ss <;> rw [h] at hok
+    case nil => apply elabStmtsA.correct.nil.sound hrefines_fm₀ hok
+    case cons s ss =>
+      apply (elabStmtsA.correct.cons s ss (elabStmtA.correct s) (elabStmtsA.correct ss)).sound
+        hrefines_fm₀ hok
+end
+
+end FlowAnalysis
