lean/FlowAnalysis/Elements.lean
@@ -1,0 +1,30 @@
+module
+public import FlowAnalysis.Types
+
+namespace FlowAnalysis
+
+variable {τ : Type} [DartTypeRepr τ]
+
+-- A local variable or function parameter.
+public structure Variable where
+  name : String
+  type : τ
+  deriving Repr, BEq, DecidableEq
+
+local notation "Variable" => Variable (τ := τ)
+
+public instance Variable.instHashable : Hashable Variable where
+  hash v := hash v.name
+
+-- Establish some properties of the `Variable` type so that it can be used as the key for a hashmap.
+public instance Variable.instLawfulBEq : LawfulBEq Variable where
+  rfl := by
+    intro v
+    simp [BEq.beq, instBEqVariable.beq]
+
+  eq_of_beq := by
+    rintro ⟨n, T⟩ ⟨n', T'⟩
+    simp [BEq.beq, instBEqVariable.beq]
+
+public instance Variable.instLawfulHashable : LawfulHashable Variable where
+  hash_eq := by simp_all
