lean/FlowAnalysis/State.lean
@@ -1,0 +1,123 @@
+module
+public import FlowAnalysis.Elements
+public import FlowAnalysis.PromotionChain
+public import FlowAnalysis.Types
+
+namespace FlowAnalysis
+
+variable {τ : Type} [DartTypeRepr τ]
+
+local notation "PromotionChain" => PromotionChain (τ := τ)
+local notation "Variable" => Variable (τ := τ)
+
+/-- A part of the program being analyzed that is a candidate for type promotion. -/
+public inductive Reference where
+  /-- A local variable. -/
+  | var (v : Variable)
+  /- TODO: promotable field, `this`, `super`. -/
+  deriving Repr, BEq
+
+local notation "Reference" => Reference (τ := τ)
+
+/-- The state of a promotable value at a particular point in a function's execution. -/
+@[ext]
+public structure ValueModel where
+  promotedTypes : PromotionChain
+
+local notation "ValueModel" => ValueModel (τ := τ)
+
+@[expose]
+public def ValueModel.currentType (vm : ValueModel) (baseType : τ) :=
+  match vm.promotedTypes.val.getLast? with
+  | none => baseType
+  | some T => if T ≤ baseType then T else baseType
+
+@[expose]
+public def ValueModel.join (vm₁ vm₂ : ValueModel) :
+    ValueModel :=
+  ⟨vm₁.promotedTypes.join vm₂.promotedTypes⟩
+
+/-- The state of a function at a particular point in its execution. -/
+@[ext]
+public structure FlowModel where
+  /-- Partial function mapping `Variable`s to type promotion information. -/
+  env : Variable → Option ValueModel
+
+local notation "FlowModel" => FlowModel (τ := τ)
+
+/-- The initial state of flow analysis. -/
+@[expose]
+public def FlowModel.empty : FlowModel := ⟨fun _ => none⟩
+
+/-- `fm.set v T` returns a modified `FlowModel` in which the type of `v` has been changed to `T`. -/
+@[expose]
+public def FlowModel.set (fm : FlowModel) (v : Variable)
+    (vm : ValueModel) : FlowModel :=
+  ⟨fun v' => if v = v' then vm else fm.env v'⟩
+
+-- TODO: implement full `join` behavior.
+@[expose]
+public def FlowModel.join (fm₁ fm₂ : FlowModel) : FlowModel :=
+  ⟨fun v =>
+     match fm₁.env v with
+     | none => none
+     | some vm₁ =>
+         match fm₂.env v with
+         | none => none
+         | some vm₂ => vm₁.join vm₂⟩
+
+-- FlowModel Theorems --
+
+@[simp]
+public theorem FlowModel.env_set {fm : FlowModel} {v v' T} :
+    (fm.set v T).env v' = if v = v' then some T else fm.env v' := by
+  simp_all [FlowModel.set]
+
+public theorem FlowModel.set_get?_neq {fm : FlowModel} {v v' : Variable}
+    {vm : ValueModel} :
+    v ≠ v' → (fm.set v vm).env v' = fm.env v' := by
+  intro hNeq
+  simp [hNeq]
+
+@[simp]
+public theorem FlowModel.get?_set {fm : FlowModel} {v v' T} :
+    (fm.set v T).env v' = if v = v' then some T else fm.env v' := by
+  simp_all [FlowModel.set]
+
+public theorem FlowModel.extensionality {fm fm' : FlowModel} :
+    (∀ v : Variable, fm.env v = fm'.env v) → fm = fm' := by
+  rcases fm; rename_i env
+  rcases fm'; rename_i env'
+  simp
+  apply funext
+
+@[simp]
+public theorem FlowModel.join_idempotent (fm : FlowModel) :
+    fm.join fm = fm := by
+  apply extensionality; intro v
+  simp [FlowModel.join]
+  cases fm.env v <;> simp_all
+  case some vm =>
+    ext; simp [ValueModel.join]
+
+instance FlowModel.instIdempotentOpJoin : Std.IdempotentOp (FlowModel.join (τ := τ)) where
+  idempotent := join_idempotent
+
+public structure ExprModel where
+  type : τ
+  ref? : Option Reference
+  fm_true : FlowModel
+  fm_false : FlowModel
+
+local notation "ExprModel" => ExprModel (τ := τ)
+
+@[expose]
+public def ExprModel.fm_after (em : ExprModel) := em.fm_true.join em.fm_false
+
+@[simp]
+public theorem ExprModel.simple_after {ref? : Option Reference} {T : τ}
+    {fm : FlowModel} :
+    (ExprModel.mk T ref? fm fm).fm_after = fm := by
+  simp [ExprModel.fm_after]
+
+end FlowAnalysis
