lean/FlowAnalysis/Syntax.lean
@@ -1,0 +1,29 @@
+module
+public import FlowAnalysis.Elements
+public import FlowAnalysis.Types
+
+namespace FlowAnalysis
+
+variable {τ : Type} [DartTypeRepr τ]
+
+local notation "Variable" => Variable (τ := τ)
+
+public inductive Expr where
+  | var (v : Variable)
+  | nullCheck (e₁ : Expr)
+  | as (e₁ : Expr) (T : τ)
+  | null
+  deriving Repr
+
+local notation "Expr" => Expr (τ := τ)
+
+public instance Expr.instToString : ToString Expr where
+  toString e := (repr e).pretty
+
+public inductive Stmt where
+  | declare (n : String) (T : τ)
+  | exprStmt (e : Expr)
+  | ifStmt (e₁ : Expr) (s₂ s₃ : Stmt)
+  | block (ss : List Stmt)
+
+end FlowAnalysis
