lean/Main.lean
@@ -1,5 +1,111 @@
 module
+public meta import FlowAnalysis.Algorithm
+public meta import FlowAnalysis.Lowered
 import FlowAnalysis
+public meta import FlowAnalysis.SimpleTypes
+import FlowAnalysis.SimpleTypes
 
+open FlowAnalysis
+open SimpleType
+
+local notation "LoweredExpr" => LoweredExpr (τ := SimpleType)
+local notation "Stmt" => Stmt (τ := SimpleType)
+local notation "Variable" => Variable (τ := SimpleType)
+
+def runFlowAnalysis (s : Stmt) : LoweredExpr ⊕ String :=
+  let loweredResult := do
+    let runResult ← elabStmtA s ⟨⟩ FlowModelA.empty
+    pure runResult.fst
+  match loweredResult with
+    | .ok m => .inl m
+    | .error s => .inr s
+
+@[simp]
+def x : Variable := ⟨"x", ObjectQ⟩
+
+def testNullAssertAST : Stmt :=
+  Stmt.block [
+    Stmt.declare "x" ObjectQ,
+    Stmt.exprStmt (Expr.nullCheck (Expr.var x)),
+    Stmt.exprStmt (Expr.var x)
+  ]
+
+def expectedNullAssertLowered : LoweredExpr :=
+  LoweredExpr.block [
+    LoweredExpr.declare x ObjectQ,
+    LoweredExpr.nullCheck (LoweredExpr.var x ObjectQ),
+    LoweredExpr.var x Object
+  ]
+
+#guard runFlowAnalysis testNullAssertAST == .inl expectedNullAssertLowered
+
+def testAsExprAST : Stmt :=
+  Stmt.block [
+    Stmt.declare "x" ObjectQ,
+    Stmt.exprStmt ((Expr.var x).as Object),
+    Stmt.exprStmt (Expr.var x)
+  ]
+
+def expectedAsExprLowered : LoweredExpr :=
+  LoweredExpr.block [
+    LoweredExpr.declare x ObjectQ,
+    (LoweredExpr.var x ObjectQ).as Object,
+    LoweredExpr.var x Object
+  ]
+
+#guard runFlowAnalysis testAsExprAST == .inl expectedAsExprLowered
+
+def testNullLiteralAST : Stmt :=
+  Stmt.block [
+    Stmt.exprStmt .null
+  ]
+
+def expectedNullLiteralLowered : LoweredExpr :=
+  LoweredExpr.block [
+    .null
+  ]
+
+#guard runFlowAnalysis testNullLiteralAST == .inl expectedNullLiteralLowered
+
+def testNullAssertAsIntAST : Stmt :=
+  Stmt.block [
+    Stmt.declare "x" ObjectQ,
+    Stmt.exprStmt ((Expr.var x).nullCheck.as int),
+    Stmt.exprStmt (Expr.var x)
+  ]
+
+def expectedNullAssertAsIntLowered : LoweredExpr :=
+  LoweredExpr.block [
+    LoweredExpr.declare x ObjectQ,
+    (LoweredExpr.nullCheck (LoweredExpr.var x ObjectQ)).as int,
+    -- The fact that `x` is typed as `Object` here rather than `int` demonstrates a sound but
+    -- limiting design choice in Dart's current flow analysis. Because `x!` outputs `none` as
+    -- its reference rather than retaining the variable reference, the outer `as int` check
+    -- cannot promote `x` any further.
+    LoweredExpr.var x Object
+  ]
+
+#guard runFlowAnalysis testNullAssertAsIntAST == .inl expectedNullAssertAsIntLowered
+
+def testAsObjectAsIntAST : Stmt :=
+  Stmt.block [
+    Stmt.declare "x" ObjectQ,
+    Stmt.exprStmt (((Expr.var x).as Object).as int),
+    Stmt.exprStmt (Expr.var x)
+  ]
+
+def expectedAsObjectAsIntLowered : LoweredExpr :=
+  LoweredExpr.block [
+    LoweredExpr.declare x ObjectQ,
+    ((LoweredExpr.var x ObjectQ).as Object).as int,
+    -- Just like with `x!`, `x as Object` outputs `none` as its reference. Thus, the outer
+    -- `as int` check receives no reference and cannot promote `x` to `int`. This is a limitation
+    -- that prevents chained promotions.
+    LoweredExpr.var x Object
+  ]
+
+#guard runFlowAnalysis testAsObjectAsIntAST == .inl expectedAsObjectAsIntLowered
+
+-- TODO: switch to tests so I don't need this.
 public def main : IO Unit := do
   IO.println "All proofs and declarations checked successfully!"
